src/Lustre/LCausality.v
@@ -10,7 +10,7 @@ From compcert Require Import common.Errors.
 From Velus Require Import Common Environment.
 From Velus Require Import Operators.
 From Velus Require Import Clocks.
-From Velus Require Import CheckGraph.
+From Velus Require Import AcyGraph.
 From Velus Require Import Lustre.LSyntax.
 
 (** * Lustre causality *)
@@ -80,17 +80,34 @@ Module Type LCAUSALITY
                                nth k xs xH = x /\
                                Is_free_left_list y k es) eqs.
 
-  Inductive Is_causal (eqs : list equation) : list ident -> Prop :=
-  | ICnil: Is_causal eqs []
-  | ICcons: forall x xs,
-      Is_causal eqs xs ->
-      (forall y, depends_on eqs x y -> In y xs) ->
-      Is_causal eqs (x::xs).
-  Hint Constructors Is_causal.
+  Definition depends_on_ck vars (eqs : list equation) (x : ident) (y : ident) :=
+    depends_on eqs x y \/ (exists ck, In (x, ck) vars /\ Is_free_in_clock y ck).
+
+  Definition graph_of_eqs {v a} vars eqs (g : AcyGraph v a) : Prop :=
+    PS.Equal (vertices g) (PSP.of_list (map fst vars)) /\
+    (forall x y, depends_on_ck vars eqs x y -> is_arc g y x).
+
+  Definition graph_of_node {v a} (n : node) (g : AcyGraph v a) : Prop :=
+    graph_of_eqs (idck (n_in n ++ n_vars n ++ n_out n)) (n_eqs n) g.
 
   Definition node_causal (n : node) :=
-    exists xs, Permutation xs (map fst (n_in n ++ n_vars n ++ n_out n))
-          /\ Is_causal (n_eqs n) xs.
+    exists {v a} (g : AcyGraph v a), graph_of_node n g.
+
+  Instance graph_of_eqs_Proper {v a} :
+    Proper (@Permutation _ ==> @Permutation _ ==> @eq (AcyGraph v a) ==> @Basics.impl)
+           graph_of_eqs.
+  Proof.
+    intros vars vars' Hp1 eqs eqs' Hp2 ? xs ? (Hv&Ha); subst.
+    split; auto.
+    - rewrite <- ps_from_list_ps_of_list in *.
+      rewrite <- Hp1; auto.
+    - intros * Hdep. apply Ha.
+      destruct Hdep as [?|(ck&?&?)].
+      + left. unfold depends_on in *.
+        rewrite Hp2; auto.
+      + right. exists ck; split; auto.
+        rewrite Hp1; auto.
+  Qed.
 
   Fact Is_free_left_list_length' : forall es x k,
       Forall (fun e => forall x k, Is_free_left x k e -> k < Datatypes.length (annot e)) es ->
@@ -155,20 +172,6 @@ Module Type LCAUSALITY
       exists k'. right; auto.
   Qed.
 
-  Instance Is_causal_Proper:
-    Proper (@Permutation equation ==> @eq (list ident) ==> iff)
-           Is_causal.
-  Proof.
-    intros eqs eqs' Hperm ? xs Heq; subst.
-    split; intros Hcaus; induction Hcaus; auto.
-    - constructor; auto.
-      intros y Hdep. apply H.
-      unfold depends_on in *. rewrite Hperm; auto.
-    - constructor; auto.
-      intros y Hdep. apply H.
-      unfold depends_on in *. rewrite <- Hperm; auto.
-  Qed.
-
   Instance vars_defined_Proper:
     Proper (@Permutation equation ==> @Permutation ident)
            vars_defined.
@@ -223,16 +226,29 @@ Module Type LCAUSALITY
   Definition collect_free_left_list (es : list exp) :=
     flat_map collect_free_left es.
 
-  Definition build_graph (n : node) : Env.t (list positive) :=
-    Env.from_list (flat_map (fun '(xs, es) =>
-                               let frees := collect_free_left_list es in
-                               List.combine xs (List.map PSP.to_list frees)) (n_eqs n)
-                            ++ (map (fun '(x, _) => (x, [])) (n_in n))).
+  Fixpoint collect_free_clock (ck : clock) : PS.t :=
+    match ck with
+    | Cbase => PS.empty
+    | Con ck x _ => (PS.add x (collect_free_clock ck))
+    end.
 
-  Definition check_node_causality (n : node) :=
-    if check_graph (build_graph n)
-    then Errors.OK tt
-    else Errors.Error (MSG "Causality error in node '" :: CTX (n_name n) :: msg "'").
+  Definition build_graph (n : node) : Env.t PS.t :=
+    let vo := flat_map (fun '(xs, es) =>
+                                 let frees := collect_free_left_list es in
+                                 List.combine xs frees) (n_eqs n) in
+    let env := Env.from_list (vo ++ (map (fun '(x, (_, ck)) => (x, PS.empty)) (n_in n))) in
+    Env.mapi (fun x deps => match List.find (fun '(x', _) => (x' =? x)%positive) (n_in n ++ n_vars n ++ n_out n) with
+                         | Some (_, (_, ck)) => PS.union deps (collect_free_clock ck)
+                         | None => deps
+                         end) env.
+
+  Open Scope error_monad_scope.
+
+  Definition check_node_causality (n : node) : res unit :=
+    match build_acyclic_graph (build_graph n) with
+    | OK _ => OK tt
+    | Error msg => Error (MSG "Node " :: (CTX (n_name n)) :: MSG " : " :: msg)
+    end.
 
   Definition check_causality (G : global) :=
     mmap check_node_causality G.
@@ -301,9 +317,230 @@ Module Type LCAUSALITY
     eapply collect_free_left_length; eauto.
   Qed.
 
+  Lemma collect_free_left_list_spec' : forall G es x k,
+      Forall (wl_exp G) es ->
+      Forall (fun e => forall k, wl_exp G e -> PS.In x (nth k (collect_free_left e) PS.empty) <-> Is_free_left x k e) es ->
+      PS.In x (List.nth k (collect_free_left_list es) PS.empty) <->
+      Is_free_left_list x k es.
+  Proof.
+    induction es; intros * Hwl Hf; inv Hwl; inv Hf.
+    - split; intros H.
+      + exfalso. eapply not_In_empty. simpl in H; destruct k; eauto.
+      + inv H.
+    - assert (length (collect_free_left a) = numstreams a) as Hlen.
+      { erewrite collect_free_left_length, length_annot_numstreams; eauto. }
+      split; intros H; simpl in *.
+      + destruct (Compare_dec.dec_lt k (numstreams a)).
+        * left; eauto.
+          rewrite app_nth1, H3 in H; eauto. congruence.
+        * apply Compare_dec.not_lt in H0.
+          right; eauto.
+          rewrite app_nth2, IHes in H; eauto. 1,2:congruence.
+      + inv H.
+        * rewrite app_nth1, H3; eauto. congruence.
+        * rewrite app_nth2, IHes; eauto. 1,2:congruence.
+  Qed.
+
+  Lemma psunion_collect_free_list_spec' : forall G es x,
+      Forall (wl_exp G) es ->
+      Forall (fun e => forall k, wl_exp G e -> PS.In x (nth k (collect_free_left e) PS.empty) <-> Is_free_left x k e) es ->
+      PS.In x (PSUnion (collect_free_left_list es)) <->
+      (exists k', Exists (Is_free_left x k') es).
+  Proof.
+    induction es; intros * Hwl Hf; inv Hwl; inv Hf; split; intros H; simpl in *.
+    - exfalso.
+      rewrite PSUnion_nil in H. apply not_In_empty in H; auto.
+    - destruct H as (?&Hex). inv Hex.
+    - rewrite PSUnion_In_app in H.
+      destruct H as [H|H].
+      + apply PSUnion_In_In in H as (?&?&?).
+        eapply In_nth in H as (?&?&Hnth).
+        rewrite <- Hnth, H3 in H0; eauto.
+      + rewrite IHes in H; eauto.
+        destruct H as (k'&Hex); eauto.
+    - rewrite PSUnion_In_app.
+      destruct H as (?&Hex). inv Hex; auto.
+      + assert (Hk:=H0).
+        eapply Is_free_left_length in Hk; eauto; erewrite <- collect_free_left_length in Hk; eauto.
+        apply H3 in H0; auto.
+        left. eapply In_In_PSUnion; eauto.
+        eapply nth_In; auto.
+      + right. rewrite IHes; eauto.
+  Qed.
+
+  Fact ps_In_k_lt : forall x l k,
+      PS.In x (nth k l PS.empty) ->
+      k < length l.
+  Proof.
+    induction l; intros * Hin; simpl in *.
+    - exfalso. eapply not_In_empty. destruct k; eauto.
+    - destruct k; eauto.
+      + apply PeanoNat.Nat.lt_0_succ.
+      + apply Lt.lt_n_S; auto.
+  Qed.
+
+  Fact collect_free_left_spec: forall G x e k,
+      wl_exp G e ->
+      PS.In x (List.nth k (collect_free_left e) PS.empty) <->
+      Is_free_left x k e.
+  Proof.
+    induction e using exp_ind2;
+      (intros * Hwl;
+       specialize (Is_free_left_length G _ x k Hwl) as Hlen1;
+       specialize (collect_free_left_length _ _ Hwl) as Hlen2;
+       try destruct a as [ty [ck name]];
+       inv Hwl; simpl in *;
+       try rewrite <- length_annot_numstreams in *; idtac).
+    - (* const *)
+      split; intros.
+      + exfalso. eapply not_In_empty. repeat (destruct k; eauto).
+      + inv H.
+    - (* var *)
+      split; intros.
+      + simpl in H. destruct k. 2:exfalso; eapply not_In_empty; destruct k; eauto.
+        apply PSF.singleton_1 in H; subst. constructor.
+      + inv H; simpl. apply PSF.singleton_2; auto.
+    - (* unop *)
+      rewrite IHe; eauto.
+      split; intros.
+      + assert (Hk:=H). eapply Is_free_left_length in Hk; eauto.
+        rewrite H4 in Hk. apply PeanoNat.Nat.lt_1_r in Hk; subst; auto.
+      + inv H. auto.
+    - (* binop *)
+      erewrite <- collect_free_left_length in H6, H7; eauto.
+      repeat singleton_length.
+      split; intros H.
+      + destruct k; [|destruct k]. 2,3:destruct (not_In_empty _ H).
+        apply PSF.union_1 in H as [?|?]; constructor.
+        * left. rewrite <- IHe1; eauto.
+        * right. rewrite <- IHe2; eauto.
+      + inv H. destruct H2 as [?|?].
+        * apply PSF.union_2. rewrite <- IHe1 in H; eauto.
+        * apply PSF.union_3. rewrite <- IHe2 in H; eauto.
+    - (* fby *)
+      rewrite collect_free_left_list_spec'; eauto.
+      split; intros; auto.
+      inv H1; auto.
+    - (* arrow *)
+      split; intros.
+      + specialize (ps_In_k_lt _ _ _ H1) as Hk. rewrite map_length in Hk.
+        erewrite map_nth' with (d':=(PS.empty, PS.empty)) in H1; eauto.
+        rewrite combine_nth in H1.
+        2:(repeat erewrite collect_free_left_list_length; eauto; rewrite H7, H8; auto).
+        rewrite PS.union_spec in H1. do 2 rewrite collect_free_left_list_spec' in H1; eauto.
+      + erewrite <- collect_free_left_list_length in H7, H8; eauto.
+        erewrite map_nth' with (d':=(PS.empty, PS.empty)).
+        2:(erewrite <- map_length, Hlen2; eauto).
+        rewrite combine_nth. 2:setoid_rewrite H7; setoid_rewrite H8; auto.
+        rewrite PS.union_spec. repeat rewrite collect_free_left_list_spec'; eauto.
+        inv H1; auto.
+    - (* when *)
+      split; intros.
+      + specialize (ps_In_k_lt _ _ _ H0) as Hk. rewrite map_length in Hk.
+        erewrite map_nth' with (d':=PS.empty) in H0; eauto.
+        constructor.
+        apply PS.add_spec in H0 as [?|?]; subst; simpl.
+        * left; split; auto.
+          erewrite collect_free_left_list_length in Hk; eauto.
+          congruence.
+        * right. rewrite <- collect_free_left_list_spec'; eauto.
+      + erewrite <- collect_free_left_list_length in H7; eauto.
+        erewrite map_nth' with (d':=PS.empty).
+        2:(erewrite <- map_length, Hlen2; eapply Hlen1; eauto).
+        inv H0. destruct H4 as [(_&?)|?]; subst.
+        * apply PSF.add_1; auto.
+        * apply PSF.add_2. erewrite collect_free_left_list_spec'; eauto.
+    - (* merge *)
+      split; intros.
+      + specialize (ps_In_k_lt _ _ _ H1) as Hk. rewrite map_length in Hk.
+        erewrite map_nth' with (d':=(PS.empty, PS.empty)) in H1; eauto.
+        rewrite combine_nth in H1.
+        2:(repeat erewrite collect_free_left_list_length; eauto; rewrite H9, H10; auto).
+        rewrite PSF.add_iff, PS.union_spec in H1. do 2 rewrite collect_free_left_list_spec' in H1; eauto.
+        constructor.
+        destruct H1 as [?|?]; subst; auto.
+        left; split; auto.
+        erewrite <- map_length, Hlen2, map_length in Hk; auto.
+      + erewrite <- collect_free_left_list_length in H9, H10; eauto.
+        erewrite map_nth' with (d':=(PS.empty, PS.empty)).
+        2:(erewrite <- map_length, Hlen2; eauto).
+        rewrite combine_nth. 2:setoid_rewrite H9; setoid_rewrite H10; auto.
+        rewrite PSF.add_iff, PS.union_spec. repeat rewrite collect_free_left_list_spec'; eauto.
+        inv H1; auto. destruct H4 as [(_&?)|?]; auto.
+    - (* ite *)
+      split; intros.
+      + specialize (ps_In_k_lt _ _ _ H1) as Hk. rewrite map_length in Hk.
+        erewrite map_nth' with (d':=(PS.empty, PS.empty)) in H1; eauto.
+        rewrite combine_nth in H1.
+        2:(repeat erewrite collect_free_left_list_length; eauto; rewrite H11, H12; auto).
+        repeat rewrite PS.union_spec in H1. do 2 rewrite collect_free_left_list_spec' in H1; eauto.
+        constructor.
+        destruct H1 as [?|?]; subst; auto.
+        left; split; auto.
+        erewrite <- map_length, Hlen2, map_length in Hk; auto.
+        rewrite <- IHe; eauto. destruct (collect_free_left _); auto.
+      + erewrite <- collect_free_left_list_length in H11, H12; eauto.
+        erewrite map_nth' with (d':=(PS.empty, PS.empty)).
+        2:(erewrite <- map_length, Hlen2; eauto).
+        rewrite combine_nth. 2:setoid_rewrite H11; setoid_rewrite H12; auto.
+        repeat rewrite PS.union_spec. repeat rewrite collect_free_left_list_spec'; eauto.
+        inv H1; auto. destruct H4 as [(_&?)|?]; auto.
+        left. rewrite <- IHe in H1; eauto.
+        destruct (collect_free_left _); auto.
+    - (* app *)
+      split; intros.
+      + assert (Hk:=H1). eapply ps_In_k_lt in Hk. rewrite map_length in Hk.
+        erewrite map_nth' in H1; eauto. 2:exact (Op.bool_type, (Cbase, None)).
+        constructor; auto.
+        rewrite <- psunion_collect_free_list_spec'; eauto.
+      + inv H1. erewrite map_nth'; eauto. 2:exact (Op.bool_type, (Cbase, None)).
+        rewrite psunion_collect_free_list_spec'; eauto.
+    - (* app (reset) *)
+      split; intros.
+      + assert (Hk:=H1). eapply ps_In_k_lt in Hk. rewrite map_length in Hk.
+        erewrite map_nth' in H1; eauto. 2:exact (Op.bool_type, (Cbase, None)).
+        constructor; auto.
+        apply PSUnion_In_app in H1 as [?|?].
+        * right. rewrite <- H; eauto.
+          erewrite <- collect_free_left_length in H8; eauto.
+          singleton_length. unfold PSUnion in H1; simpl in H1; auto.
+        * left. rewrite <- psunion_collect_free_list_spec'; eauto.
+      + inv H1. erewrite map_nth'; eauto. 2:exact (Op.bool_type, (Cbase, None)).
+        rewrite PSUnion_In_app.
+        destruct H14.
+        * right. rewrite psunion_collect_free_list_spec'; eauto.
+        * left. rewrite <- H in H1; eauto.
+          eapply In_In_PSUnion; eauto.
+          eapply nth_In. erewrite collect_free_left_length, H8; eauto.
+  Qed.
+
+  Corollary collect_free_left_list_spec : forall G es x k,
+      Forall (wl_exp G) es ->
+      PS.In x (List.nth k (collect_free_left_list es) PS.empty) <->
+      Is_free_left_list x k es.
+  Proof.
+    intros * Hwl.
+    eapply collect_free_left_list_spec'; eauto.
+    eapply Forall_impl; eauto; intros.
+    eapply collect_free_left_spec; eauto.
+  Qed.
+
+  Hint Constructors Is_free_in_clock.
+  Lemma collect_free_clock_spec : forall ck x,
+      PS.In x (collect_free_clock ck) <->
+      Is_free_in_clock x ck.
+  Proof.
+    induction ck; intros x; simpl; (split; [intros H|intros H; inv H]).
+    - exfalso. apply not_In_empty in H; auto.
+    - apply PSF.add_iff in H as [?|?]; subst; auto.
+      right. rewrite <- IHck; auto.
+    - apply PSF.add_1; auto.
+    - apply PSF.add_2. rewrite IHck; auto.
+  Qed.
+
   Fact wl_node_vars_defined : forall G n,
       wl_node G n ->
-      map fst (flat_map (fun '(xs, es) => combine xs (map PSP.to_list (collect_free_left_list es))) (n_eqs n)) =
+      map fst (flat_map (fun '(xs, es) => combine xs (collect_free_left_list es)) (n_eqs n)) =
       vars_defined (n_eqs n).
   Proof.
     intros * Hwl.
@@ -311,7 +548,7 @@ Module Type LCAUSALITY
     destruct x as [xs es].
     rewrite map_app, IHHwl. f_equal; auto; simpl.
     apply combine_map_fst'; auto.
-    inv H. erewrite map_length, collect_free_left_list_length; eauto.
+    inv H. erewrite collect_free_left_list_length; eauto.
   Qed.
 
   Lemma build_graph_dom : forall G n,
@@ -319,20 +556,14 @@ Module Type LCAUSALITY
       Env.dom (build_graph n) (map fst (n_in n ++ n_vars n ++ n_out n)).
   Proof.
     intros * Hwl. unfold build_graph.
-    eapply Env.dom_Permutation.
-    2:{ eapply Env.dom_from_list_map_fst; eauto.
-        rewrite fst_NoDupMembers, map_app.
-        setoid_rewrite wl_node_vars_defined; eauto. rewrite n_defd.
-        replace (map fst (map (fun '(x, _) => (x, [])) (n_in n))) with (map fst (n_in n)).
-        rewrite Permutation_app_comm.
-        rewrite <- map_app. apply node_NoDup.
-        rewrite map_map. eapply map_ext; intros [? ?]; auto.
-    }
-    repeat rewrite map_app. setoid_rewrite wl_node_vars_defined; eauto.
-    rewrite (Permutation_app_comm (map _ (n_vars n))), n_defd, map_app, Permutation_app_comm, (Permutation_app_comm (map _ (n_out _))).
-    eapply Permutation_app_head.
-    replace (map fst (map (fun '(x, _) => (x, [])) (n_in n))) with (map fst (n_in n)); auto.
-    rewrite map_map. eapply map_ext; intros [? ?]; auto.
+    eapply Env.dom_intro. intros x.
+    rewrite Env.Props.P.F.mapi_in_iff.
+    rewrite Env.In_from_list, fst_InMembers.
+    repeat rewrite map_app. repeat rewrite map_map.
+    rewrite Permutation_app_comm.
+    erewrite map_ext with (g:=fst). 2:intros (?&?&?); auto.
+    setoid_rewrite wl_node_vars_defined; eauto.
+    rewrite n_defd, map_app. reflexivity.
   Qed.
 
   Corollary build_graph_Perm : forall G n,
@@ -347,175 +578,68 @@ Module Type LCAUSALITY
     - apply node_NoDup.
   Qed.
 
-  Lemma build_graph_find' : forall G n,
+  Fact find_some' : forall {A} (xs : list (ident * A)) x v ,
+      NoDupMembers xs ->
+      In (x, v) xs ->
+      find (fun '(x', _) => (x' =? x)%positive) xs = Some (x, v).
+  Proof.
+    induction xs; intros * Hndup Hin; inv Hin; inv Hndup; simpl.
+    - rewrite Pos.eqb_refl. reflexivity.
+    - destruct (ident_eq_dec a0 x); subst.
+      + apply In_InMembers in H. contradiction.
+      + eapply Pos.eqb_neq in n. rewrite n; auto.
+  Qed.
+
+  Lemma build_graph_find : forall G n x y,
       wl_node G n ->
-      Forall (fun x => forall k xs es,
-                  In (xs, es) (n_eqs n) ->
-                  k < List.length xs ->
-                  nth k xs xH = x ->
-                  Env.find x (build_graph n) = Some (List.nth k (map PSP.to_list (collect_free_left_list es)) []))
-             (map fst (n_in n ++ n_vars n ++ n_out n)).
+      depends_on_ck (idck (n_in n ++ n_vars n ++ n_out n)) (n_eqs n) x y ->
+      exists ys, (Env.find x (build_graph n)) = Some ys /\ PS.In y ys.
   Proof.
-    intros * Hwl.
-    rewrite Forall_forall.
-    intros ? Hx ? ? ? Heq Hk Hnth.
-    unfold build_graph.
-    eapply Env.find_In_from_list.
-    2:{ rewrite fst_NoDupMembers, map_app.
-        setoid_rewrite wl_node_vars_defined; eauto. rewrite n_defd.
-        replace (map fst (map (fun '(x, _) => (x, [])) (n_in n))) with (map fst (n_in n)).
-        rewrite Permutation_app_comm.
-        rewrite <- map_app. apply node_NoDup.
-        rewrite map_map. eapply map_ext; intros [? ?]; auto.
-    }
-    rewrite in_app_iff; left.
-    rewrite in_flat_map. exists (xs, es); split; auto.
-    assert (Datatypes.length xs = Datatypes.length (map PSP.to_list (collect_free_left_list es))) as Hlen.
-    { eapply Forall_forall in Hwl; eauto. inv Hwl.
-      erewrite map_length, collect_free_left_list_length; eauto. }
-    rewrite <- Hnth, <- combine_nth; auto.
-    eapply nth_In. rewrite combine_length, <- Hlen, PeanoNat.Nat.min_id; auto.
-  Qed.
-
-  Corollary collect_free_left_list_complete' : forall G es x k,
-      Forall (wl_exp G) es ->
-      Forall (fun e => forall x k, Is_free_left x k e -> PS.In x (List.nth k (collect_free_left e) PS.empty)) es ->
-      Is_free_left_list x k es ->
-      PS.In x (List.nth k (collect_free_left_list es) PS.empty).
-  Proof.
-    induction es; intros * Hwl Hf Hfree; inv Hwl; inv Hf. inv Hfree.
-    assert (length (collect_free_left a) = numstreams a) as Hlen.
-    { erewrite collect_free_left_length, length_annot_numstreams; eauto. }
-    inv Hfree; simpl.
-    - rewrite app_nth1; eauto. congruence.
-    - rewrite app_nth2; eauto.
-      + eapply IHes; eauto. congruence.
-      + congruence.
-  Qed.
-
-  Fact collect_free_left_complete : forall G e x k,
-      wl_exp G e ->
-      Is_free_left x k e ->
-      PS.In x (List.nth k (collect_free_left e) PS.empty).
-  Proof.
-    Ltac solve_forall3 Hfree H :=
-      eapply collect_free_left_list_complete' in Hfree; eauto;
-      eapply Forall_Forall in H; eauto; eapply Forall_impl; eauto; intros ? [? ?] ? ? ?; auto.
-
-    induction e using exp_ind2;
-      (intros * Hwl Hfree;
-       assert (Hk := Hfree); eapply Is_free_left_length in Hk; eauto;
-       try destruct a as [ty [ck name]];
-       inv Hfree; inv Hwl; simpl in *;
-       try rewrite <- length_annot_numstreams in *).
-    - (* var *)
-      apply PSF.singleton_2; auto.
-    - (* unop *) eauto.
-    - (* binop *)
-      erewrite <- collect_free_left_length in H7, H8; eauto.
-      erewrite map_nth' with (d':=(PS.empty, PS.empty)).
-      2:(rewrite combine_length; rewrite H7, H8, PeanoNat.Nat.min_id; eauto).
-      rewrite combine_nth. 2:congruence.
-      rewrite PS.union_spec. destruct H1; eauto.
-    - (* fby *)
-      eapply collect_free_left_list_complete'; eauto.
-      solve_forall3 H3 H.
-    - (* arrow *)
-      erewrite <- collect_free_left_list_length in H8, H9; eauto.
-      erewrite map_nth' with (d':=(PS.empty, PS.empty)).
-      2:(rewrite combine_length; setoid_rewrite H8; setoid_rewrite H9; rewrite PeanoNat.Nat.min_id; eauto).
-      rewrite combine_nth. 2:setoid_rewrite H8; setoid_rewrite H9; auto.
-      rewrite PS.union_spec.
-      destruct H3 as [Hfree|Hfree]. solve_forall3 Hfree H. solve_forall3 Hfree H0.
-    - (* when *)
-      rewrite map_length in Hk. erewrite <- collect_free_left_list_length in H8; eauto.
-      erewrite map_nth' with (d':=PS.empty). 2:setoid_rewrite H8; auto.
-      rewrite PS.add_spec. destruct H2 as [[? ?]|Hfree]; auto.
-      solve_forall3 Hfree H.
-    - (* merge *)
-      rewrite map_length in Hk. erewrite <- collect_free_left_list_length in H10, H11; eauto.
-      erewrite map_nth' with (d':=(PS.empty,PS.empty)).
-      2:(rewrite combine_length; setoid_rewrite H10; setoid_rewrite H11; rewrite PeanoNat.Nat.min_id; eauto).
-      rewrite combine_nth. 2:setoid_rewrite H10; setoid_rewrite H11; auto.
-      rewrite PS.add_spec, PS.union_spec.
-      destruct H3 as [[? ?]|[Hfree|Hfree]]; auto. solve_forall3 Hfree H. solve_forall3 Hfree H0.
-    - (* ite *)
-      rewrite map_length in Hk. erewrite <- collect_free_left_list_length in H12, H13; eauto.
-      erewrite map_nth' with (d':=(PS.empty,PS.empty)).
-      2:(rewrite combine_length; setoid_rewrite H12; setoid_rewrite H13; rewrite PeanoNat.Nat.min_id; eauto).
-      rewrite combine_nth. 2:setoid_rewrite H12; setoid_rewrite H13; auto.
-      rewrite PS.union_spec, PS.union_spec.
-      destruct H3 as [[? ?]|[Hfree|Hfree]]; auto. 2:solve_forall3 Hfree H. 2:solve_forall3 Hfree H0.
-      left. eapply IHe in H2; eauto.
-      destruct (collect_free_left e); auto.
-    - (* app *)
-      erewrite map_nth'; eauto. 2:exact (Op.bool_type, (Cbase, None)).
-      destruct H7 as [k' Hex]. apply Exists_exists in Hex as [e [Hin Hfree]].
-      eapply Forall_forall in H0; eauto. eapply Forall_forall in H5; eauto.
-      specialize (H0 _ _ H5 Hfree).
-      eapply In_In_PSUnion; eauto.
-      rewrite flat_map_concat_map. eapply incl_concat_map; eauto.
-      eapply nth_In. erewrite collect_free_left_length; eauto.
-      eapply Is_free_left_length in Hfree; eauto.
-    - (* app (reset) *)
-      erewrite map_nth'; eauto. 2:exact (Op.bool_type, (Cbase, None)).
-      rewrite PSUnion_In_app.
-      destruct H7 as [[k' Hex]|Hex].
-      + right. apply Exists_exists in Hex as [e [Hin Hfree]].
-        eapply Forall_forall in H0; eauto. eapply Forall_forall in H8; eauto.
-        specialize (H0 _ _ H8 Hfree).
-        eapply In_In_PSUnion; eauto.
-        rewrite flat_map_concat_map. eapply incl_concat_map; eauto.
-        eapply nth_In. erewrite collect_free_left_length; eauto.
-        eapply Is_free_left_length in Hfree; eauto.
-      + left. assert (Hfree:=Hex). eapply H in Hex; eauto.
-        eapply In_In_PSUnion; eauto.
-        eapply nth_In. erewrite collect_free_left_length; eauto.
-        eapply Is_free_left_length; eauto.
-  Qed.
-
-  Corollary collect_free_left_list_complete : forall G es x k,
-      Forall (wl_exp G) es ->
-      Is_free_left_list x k es ->
-      PS.In x (List.nth k (collect_free_left_list es) PS.empty).
-  Proof.
-    intros * Hwl Hfree.
-    eapply collect_free_left_list_complete'; eauto.
-    eapply Forall_impl; eauto; intros.
-    eapply collect_free_left_complete; eauto.
-  Qed.
-
-  Lemma build_graph_find : forall G n,
-      wl_node G n ->
-      Forall (fun x => forall y ys,
-                  depends_on (n_eqs n) x y ->
-                  (Env.find x (build_graph n)) = Some ys ->
-                  In y ys) (map fst (n_in n ++ n_vars n ++ n_out n)).
-  Proof.
-    intros * Hwl.
-    specialize (build_graph_find' _ _ Hwl) as Hfind'.
-    eapply Forall_impl; eauto; clear Hfind'.
-    intros ? Hfind ? ? Hdep Hfind'; simpl in *.
-    unfold depends_on in Hdep.
-    apply Exists_exists in Hdep as [[? ?] [Hin [k [Hk [Hnth Hfree]]]]].
-    specialize (Hfind _ _ _ Hin Hk Hnth).
-    rewrite Hfind in Hfind'. inv Hfind'.
-    eapply Forall_forall in Hwl; eauto. inv Hwl.
-    eapply collect_free_left_list_complete in Hfree; eauto.
-    erewrite map_nth' with (d':=PS.empty). 2:erewrite collect_free_left_list_length, <- H0; eauto.
-    rewrite In_PS_elements; auto.
-  Qed.
-
-  Fact WellOrdered_Is_causal : forall graph eqs xs,
-      Forall (fun x => forall y ys,
-                  depends_on eqs x y ->
-                  (Env.find x graph) = Some ys ->
-                  In y ys) xs ->
-      WellOrdered graph xs ->
-      Is_causal eqs xs.
-  Proof.
-    intros * Hconn Hord.
-    induction xs; inv Hord; inv Hconn; constructor; auto.
+    intros * Hwl Hdep.
+    specialize (build_graph_dom G n Hwl) as Hdom.
+    eapply Env.dom_use with (x0:=x) in Hdom.
+    rewrite Env.In_find in Hdom. symmetry in Hdom.
+    destruct Hdep as [Hdep|(ck&Hin&Hfree)].
+    - apply Exists_exists in Hdep as ((xs&es)&Hin&k&Hk&Hnth&Hfree).
+      assert (In x (map fst (n_in n ++ n_vars n ++ n_out n))) as Hin'.
+      { rewrite map_app. apply in_or_app; right.
+        rewrite <- n_defd. unfold vars_defined.
+        rewrite flat_map_concat_map. eapply in_concat'; eauto; subst.
+        + eapply nth_In; eauto.
+        + eapply in_map_iff. exists (xs, es); auto.
+      }
+      apply Hdom in Hin' as (?&Hfind). clear Hdom.
+      eexists; split; eauto.
+      unfold build_graph in Hfind.
+      rewrite FMapPositive.PositiveMap.gmapi in Hfind.
+      apply option_map_inv_Some in Hfind as (?&Hfind&?).
+      erewrite Env.find_In_from_list with (v:=List.nth k (collect_free_left_list es) PS.empty) in Hfind.
+      + eapply Forall_forall in Hwl; eauto. inv Hwl.
+        inv Hfind. destruct find as [(?&?&?)|]. apply PSF.union_2.
+        1,2:eapply collect_free_left_list_spec; eauto.
+      + apply in_or_app; left. rewrite in_flat_map.
+        eexists; split; eauto; simpl.
+        assert (Datatypes.length xs = Datatypes.length (collect_free_left_list es)) as Hlen.
+      { eapply Forall_forall in Hwl; eauto. inv Hwl.
+        erewrite collect_free_left_list_length; eauto. }
+      rewrite <- Hnth, <- combine_nth; auto.
+      eapply nth_In. rewrite combine_length, <- Hlen, PeanoNat.Nat.min_id; auto.
+      + rewrite fst_NoDupMembers, map_app.
+        erewrite wl_node_vars_defined; eauto.
+        rewrite map_map. erewrite map_ext with (g:=fst). 2:intros (?&?&?); auto.
+        rewrite Permutation_app_comm, n_defd, <- map_app.
+        apply node_NoDup.
+    - apply In_idck_exists in Hin as (ty&Hin).
+      assert (In x (map fst (n_in n ++ n_vars n ++ n_out n))) as Hin'.
+      { rewrite in_map_iff. exists (x, (ty, ck)); split; auto. }
+      apply Hdom in Hin' as (?&Hfind).
+      eexists; split; eauto.
+      unfold build_graph in Hfind.
+      rewrite FMapPositive.PositiveMap.gmapi in Hfind.
+      apply option_map_inv_Some in Hfind as (?&Hfind&?).
+      erewrite find_some' in H; eauto; simpl in *; subst.
+      2:apply fst_NoDupMembers, node_NoDup.
+      apply PSF.union_3. rewrite collect_free_clock_spec; auto.
   Qed.
 
   Lemma check_node_causality_correct : forall G n,
@@ -525,14 +649,16 @@ Module Type LCAUSALITY
   Proof.
     intros * Hwl Hcheck.
     unfold check_node_causality in Hcheck.
-    destruct (check_graph _) eqn:Hcheck'; inv Hcheck.
-    eapply check_graph_spec in Hcheck' as [xs [Hperm Hord]].
-    assert (Permutation xs (map fst (n_in n ++ n_vars n ++ n_out n))) as Hperm'.
-    { rewrite <- Hperm. eapply build_graph_Perm; eauto. }
-    exists xs. split; auto.
-    eapply WellOrdered_Is_causal; eauto.
-    rewrite Hperm'.
-    eapply build_graph_find; eauto.
+    destruct (build_acyclic_graph _); inv Hcheck.
+    destruct s as (v&a&g&(Hv&Ha)); simpl in *.
+    exists v. exists a. exists g. split.
+    - intros x. rewrite <- Hv.
+      apply build_graph_dom in Hwl.
+      rewrite (Hwl x), <- ps_from_list_ps_of_list, ps_from_list_In, map_fst_idck.
+      reflexivity.
+    - intros x y Hdep.
+      apply Ha.
+      eapply build_graph_find; eauto.
   Qed.
 
   Corollary check_causality_correct : forall G tts,
@@ -552,23 +678,24 @@ Module Type LCAUSALITY
   (** *** Consequence of causality.
       We can "follow the trail" of variables *)
 
-  Lemma Is_causal_inv : forall eqs x xs,
-      Is_causal eqs (x::xs) ->
+  Lemma Prefix_inv {v a} : forall (g : AcyGraph v a) eqs x xs,
+      (forall x y, depends_on eqs x y -> is_arc g y x) ->
+      Prefix g (x::xs) ->
       In x (vars_defined eqs) ->
       Exists (fun '(xs', es) =>
                 exists k, k < length xs' /\ nth k xs' xH = x /\
                      (forall y, Is_free_left_list y k es -> In y xs)
              ) eqs.
   Proof.
-    intros * Hcaus Hin.
-    inv Hcaus.
+    intros * Hdep Hpref Hin.
+    inversion_clear Hpref as [|?? (?&?&?) ?].
     unfold vars_defined in Hin.
     apply in_flat_map in Hin as [[xs' es] [Hin Hin']]; simpl in Hin'.
     eapply Exists_exists. exists (xs', es); split; eauto.
     apply In_nth with (d:=xH) in Hin' as [k [Hlen Hnth]].
     exists k. repeat split; auto.
-    intros y Hfree.
-    apply H2. unfold depends_on.
+    intros y' Hfree.
+    apply H1. left. apply Hdep. unfold depends_on.
     eapply Exists_exists. exists (xs', es); split; eauto.
   Qed.
 
@@ -746,29 +873,39 @@ Module Type LCAUSALITY
     Hypothesis Inputs :
       Forall P_var (map fst (n_in n)).
 
-    Lemma causal_ind : forall xs,
+    Lemma causal_ind {v a} : forall (g : AcyGraph v a),
         Forall (wl_equation G) (n_eqs n) ->
-        incl xs (map fst (n_in n) ++ vars_defined (n_eqs n)) ->
-        Is_causal (n_eqs n) xs ->
-        Forall P_var xs.
+        graph_of_node n g ->
+        Forall P_var (PS.elements (vertices g)).
     Proof.
-      intros * Hwl Hincl Hcaus.
-      induction xs; auto.
+      intros * Hwl [Hv Ha].
+      specialize (has_Prefix g) as (xs'&Heq&Hpre).
+      rewrite Heq, <- PS_For_all_Forall, <- ps_from_list_ps_of_list, PS_For_all_Forall'.
+      assert (incl xs' (map fst (n_in n) ++ vars_defined (n_eqs n))) as Hincl.
+      { rewrite Hv in Heq.
+        repeat rewrite <- ps_from_list_ps_of_list in Heq.
+        intros ? Hin. rewrite <- ps_from_list_In in *.
+        rewrite <- Heq, map_fst_idck, map_app in Hin.
+        rewrite n_defd. assumption. }
+      clear Heq.
+      induction xs'; auto.
       apply incl_cons' in Hincl as [HIn Hincl].
-      assert (Forall P_var xs) as Hxs by (inv Hcaus; auto).
+      assert (Forall P_var xs') as Hxs by (inv Hpre; auto).
       constructor; auto.
       apply in_app_or in HIn as [HIn|HIn].
       - (* a is in the inputs *)
         eapply Forall_forall; [|eauto]. apply Inputs.
       - (* a is in the lhs of an equation *)
-        eapply Is_causal_inv in Hcaus; eauto.
-        apply Exists_exists in Hcaus as [[xs' es] (?&k&Hk&Hnth&Hfree)]; subst.
+        eapply Prefix_inv in Hpre; eauto.
+        apply Exists_exists in Hpre as [(?&?) (?&k&Hk&Hnth&Hfree)]; subst.
         eapply EqVars; eauto.
         eapply Forall_forall in Hwl; eauto. inv Hwl.
         eapply Pexp_Pexps; eauto. 3:rewrite <- H1; auto.
         + eapply Forall_impl; eauto. intros.
           eapply exp_causal_ind; eauto.
         + intros. eapply Forall_forall in Hxs; eauto.
+        + intros * Hdep.
+          apply Ha. left; auto.
     Qed.
 
     Corollary node_causal_ind :
@@ -776,11 +913,11 @@ Module Type LCAUSALITY
         node_causal n ->
         Forall P_var (map fst (n_in n ++ n_vars n ++ n_out n)).
     Proof.
-      intros * Hwl Hcaus.
-      destruct Hcaus as [xs [Hperm Hcaus]].
-      eapply causal_ind in Hcaus; eauto.
-      - rewrite <- Hperm; auto.
-      - rewrite n_defd, <- map_app, Hperm. reflexivity.
+      intros * Hwl (?&?&g&Hcaus).
+      assert (Hvars:=Hcaus). eapply causal_ind in Hvars; eauto.
+      destruct Hcaus as (Heq&_).
+      rewrite <- PS_For_all_Forall in Hvars.
+      rewrite <- PS_For_all_Forall', ps_from_list_ps_of_list, <- map_fst_idck, <- Heq; auto.
     Qed.
 
     (** Bonus : now that the induction is done, this is true for any exp or equation *)
@@ -804,12 +941,176 @@ Module Type LCAUSALITY
 
   End causal_ind.
 
+  (** We can give a slightly stricter graph : there are arcs between two variables
+      only and only if there is actually a dependency in the node *)
+  Section strict_graph.
+
+    Definition graph_of_eqs_strict {v a} vars eqs (g : AcyGraph v a) : Prop :=
+      PS.Equal (vertices g) (PSP.of_list (map fst vars)) /\
+      (forall x y, depends_on_ck vars eqs x y <-> is_arc g y x).
+
+    (** Decidability of depends_on *)
+    Fixpoint depends_on_eqb x y xs es n :=
+      match n with
+      | O => false
+      | S n => orb (andb (ident_eqb x (nth n xs xH)) (PS.mem y (nth n (collect_free_left_list es) PS.empty)))
+                  (depends_on_eqb x y xs es n)
+      end.
+
+    Fact lt_S_n_inv : forall m n,
+        m < S n ->
+        m = n \/ m < n.
+    Proof.
+      induction m; intros * Hlt.
+      - destruct n; auto.
+        right. apply PeanoNat.Nat.lt_0_succ.
+      - apply Lt.lt_S_n in Hlt.
+        assert (0 < n) as Hn0.
+        { destruct n; auto. inv Hlt. apply PeanoNat.Nat.lt_0_succ. }
+        rewrite Lt.S_pred_pos with (n:=n) in Hlt; auto.
+        specialize (IHm _ Hlt) as [?|?]; subst.
+        + left. rewrite <- Lt.S_pred_pos; auto.
+        + right. rewrite PeanoNat.Nat.lt_succ_lt_pred; auto.
+    Qed.
+
+    Fact depends_on_eqb_spec : forall G x y xs es n,
+        wl_equation G (xs, es) ->
+        depends_on_eqb x y xs es n = true <->
+        exists k, k < n /\ nth k xs xH = x /\ Is_free_left_list y k es.
+    Proof.
+      induction n; intros Hwl; simpl;
+        (split; [intros Hdep|intros (k&Hn&Hnth&Hfree)]).
+      - inv Hdep.
+      - exfalso. apply OrdersEx.Nat_as_OT.nlt_0_r in Hn; auto.
+      - rewrite Bool.orb_true_iff, Bool.andb_true_iff in Hdep.
+        destruct Hdep as [(?&?)|?].
+        + rewrite ident_eqb_eq in H.
+          rewrite <- PSF.mem_iff, collect_free_left_list_spec in H0; eauto.
+          inv Hwl; eauto.
+        + apply IHn in H as (?&?&?&?); auto.
+          exists x0. repeat split; auto.
+      - rewrite Bool.orb_true_iff, Bool.andb_true_iff, IHn; auto.
+        destruct (lt_S_n_inv _ _ Hn); subst.
+        + left. rewrite ident_eqb_eq, <- PSF.mem_iff.
+          split; auto.
+          rewrite collect_free_left_list_spec; auto. inv Hwl; eauto.
+        + right. exists k. repeat split; auto.
+    Qed.
+
+    Lemma Is_free_in_clock_dec : forall x ck,
+        {Is_free_in_clock x ck} + {~Is_free_in_clock x ck}.
+    Proof.
+      induction ck; intros.
+      - right. intro contra. inv contra.
+      - destruct IHck.
+        + left. right; auto.
+        + destruct (ident_eq_dec x i); subst; auto.
+          right. intro contra.
+          inv contra; auto.
+    Qed.
+
+    Lemma depends_on_dec : forall G eqs,
+        Forall (wl_equation G) eqs ->
+        forall x y, {depends_on eqs x y} + {~depends_on eqs x y}.
+    Proof.
+      intros * Hwl *.
+      unfold depends_on. eapply Exists_dec_In.
+      intros (xs&es) Hin.
+      eapply Forall_forall in Hwl; eauto.
+      destruct (depends_on_eqb x y xs es (length xs)) eqn:Hdep.
+      - left. rewrite depends_on_eqb_spec in Hdep; eauto.
+      - right.
+        intro contra. rewrite <- depends_on_eqb_spec in contra; eauto.
+        congruence.
+    Qed.
+
+    Lemma in_map_fst {A B} : forall (l : list (A * B)) x,
+        (forall (x y : A), {x = y} + {x <> y}) ->
+        In x (map fst l) ->
+        { y | In (x, y) l }.
+    Proof.
+      induction l as [|(?&?) ?]; intros * Hdec Hin; simpl in *.
+      - inv Hin.
+      - destruct (Hdec a x); subst; auto.
+        + exists b; auto.
+        + specialize (IHl x Hdec).
+          destruct IHl as (?&?); eauto.
+          inv Hin; auto. congruence.
+    Qed.
+
+    Corollary depends_on_ck_dec : forall G vars eqs,
+        NoDupMembers vars ->
+        Forall (wl_equation G) eqs ->
+        forall x y, {depends_on_ck vars eqs x y} + {~depends_on_ck vars eqs x y}.
+    Proof.
+      intros * Hnd Hwl ??.
+      destruct (depends_on_dec _ _ Hwl x y).
+      - left. left. assumption.
+      - destruct (in_dec ident_eq_dec x (map fst vars)).
+        + apply in_map_fst in i as (ck&?). 2:apply ident_eq_dec.
+          destruct (Is_free_in_clock_dec y ck).
+          * left. right; eauto.
+          * right. intro contra.
+            inv contra; auto. destruct H as (?&Hin&?).
+            eapply NoDupMembers_det in i; eauto; subst. eauto.
+        + right. intro contra.
+          inv contra; auto. destruct H as (?&Hin&?).
+          eapply In_InMembers, fst_InMembers in Hin; eauto.
+    Qed.
+
+    Lemma graph_of_eqs_graph_of_eqs_strict : forall {v a} G vars eqs (g : AcyGraph v a),
+        NoDupMembers vars ->
+        Forall (wl_equation G) eqs ->
+        graph_of_eqs vars eqs g ->
+        exists a' (g' : AcyGraph v a'), graph_of_eqs_strict vars eqs g'.
+    Proof.
+      intros * Hnd Hwl (Hv&Ha).
+      specialize (depends_on_ck_dec _ vars _ Hnd Hwl) as Hdec.
+
+      (* First, we can produce a new arc_set with all the useless arcs removed *)
+      remember (Env.mapi (fun x => PS.filter (fun y => if Hdec y x then true else false)) a) as a'.
+
+      (* We can build an AcyGraph out of it *)
+      assert (exists a'', (forall x y, has_arc a'' x y <-> has_arc a' x y) /\ AcyGraph v a'') as (a''&Heq&g'').
+      { eapply subset_AcyGraph with (a':=a'); eauto.
+        subst. intros x y (?&Hmap&Hin).
+        apply Env.Props.P.F.mapi_inv in Hmap as (s&?&?&?&?); subst.
+        apply PSF.filter_1 in Hin. 2:intros ???; subst; auto.
+        exists s. auto.
+      }
+      exists a''. exists g''.
+
+      (* Every necessary arc is inside a'' *)
+      assert (forall x y, depends_on_ck vars eqs y x -> has_arc a'' x y) as Ha1.
+      { intros * Hdep. rewrite Heq; subst.
+        specialize (Ha _ _ Hdep) as (s&Hmap&Hin).
+        eapply Env.mapi_1 in Hmap as (?&?&Hmap); subst.
+        eexists; split; eauto; simpl.
+        apply PSF.filter_3; auto. 1:intros ???; subst; auto.
+        rewrite H. destruct Hdec; auto.
+      }
+
+      (* Every unnecessary arc has been removed from a'' *)
+      assert (forall x y, has_arc a'' x y -> depends_on_ck vars eqs y x) as Ha2.
+      { intros * Ha''. rewrite Heq in Ha''; subst.
+        destruct Ha'' as (?&Hmap&Hin).
+        apply Env.Props.P.F.mapi_inv in Hmap as (?&?&?&?&?); subst.
+        apply PSF.filter_2 in Hin. 2:intros ???; subst; auto.
+        destruct Hdec; auto. congruence.
+      }
+
+      split; auto. unfold is_arc.
+      intros *; split; auto.
+    Qed.
+
+  End strict_graph.
+
 End LCAUSALITY.
 
-Module LCausality
+Module LCausalityFun
        (Ids  : IDS)
        (Op   : OPERATORS)
        (Syn  : LSYNTAX Ids Op)
        <: LCAUSALITY Ids Op Syn.
   Include LCAUSALITY Ids Op Syn.
-End LCausality.
+End LCausalityFun.
