src/AcyGraph.v
@@ -1,0 +1,1220 @@
+From Coq Require Import String.
+From Coq Require Import List.
+Import List.ListNotations.
+Open Scope list_scope.
+
+From Coq Require Import RelationClasses.
+
+From Velus Require Import Common.
+From Velus Require Import Environment.
+
+Import Coq.Relations.Relation_Operators.
+
+(** ** Vertices and arcs *)
+
+(** Vertices *)
+Definition V_set : Type := PS.t.
+
+(** Arcs *)
+Definition A_set : Type := Env.t PS.t.
+
+Definition empty_arc_set : A_set := Env.empty _.
+
+(** There is an arc between x and y in the arc set *)
+Definition has_arc (a : A_set) (x y : ident) :=
+  exists s, Env.MapsTo x s a /\ PS.In y s.
+
+(** Decision procedure to find if an arc exists *)
+Definition has_arcb (a : A_set) (x y : ident) :=
+  match (Env.find x a) with
+  | Some s => PS.mem y s
+  | None => false
+  end.
+
+Lemma has_arcb_spec : forall a x y,
+    has_arcb a x y = true <-> has_arc a x y.
+Proof.
+  intros a x y.
+  unfold has_arcb, has_arc.
+  split; [intros H|intros (?&Hmap&Hin)]; destruct (Env.find _ _) eqn:Hfind.
+  - eauto.
+  - inv H.
+  - rewrite Hmap in Hfind. inv Hfind.
+    apply PSF.mem_1; auto.
+  - rewrite Hmap in Hfind. inv Hfind.
+Qed.
+
+Lemma nhas_arc_empty : forall x y,
+    ~has_arc empty_arc_set x y.
+Proof.
+  intros * (?&Hmap&_).
+  rewrite Env.Props.P.F.empty_mapsto_iff in Hmap; auto.
+Qed.
+
+(** Add a single arc *)
+Definition add_arc (x y : ident) (a : A_set) :=
+  match (Env.find x a) with
+  | Some s => Env.add x (PS.add y s) a
+  | None => Env.add x (PS.singleton y) a
+  end.
+
+Lemma add_arc_spec : forall a x y x' y',
+    has_arc (add_arc x y a) x' y' <->
+    has_arc a x' y' \/
+    (x = x' /\ y = y').
+Proof.
+  intros *. unfold add_arc, has_arc, Env.MapsTo in *.
+  split; intros H;
+    [(destruct H as (s&Hm&Hin);
+      (destruct (ident_eq_dec x x'), (ident_eq_dec y y'); subst;
+       destruct (Env.find _ a) eqn:Hfind))
+    |(destruct H as [(?&?&?)|(?&?)]; destruct (Env.find x a) eqn:Hfind; subst)].
+  1-2:right; auto.
+  1-6:left.
+  1-2:rewrite Env.gss in Hm; inv Hm.
+  3-6:rewrite Env.gso in Hm; eauto.
+  3,4:destruct (ident_eq_dec x x'), (ident_eq_dec y y'); subst.
+  1-12:try rewrite Env.gss; try rewrite Env.gso; eauto.
+  3-8:eexists; split; eauto.
+  3,7:apply PSF.add_1; auto.
+  4,6:apply PSF.singleton_2; auto.
+  - rewrite PSF.add_neq_iff in Hin; eauto.
+  - apply PSF.singleton_1 in Hin. contradiction.
+  - rewrite H in Hfind. inv Hfind. apply PSF.add_2; auto.
+  - rewrite H in Hfind. congruence.
+Qed.
+
+(** Get the successors of a vertex *)
+Definition get_succ (x : ident) (a : A_set) :=
+  match (Env.find x a) with
+  | Some s => s
+  | None => PS.empty
+  end.
+
+Lemma get_succ_spec : forall a x y,
+    PS.In y (get_succ x a) <->
+    has_arc a x y.
+Proof.
+  intros *.
+  unfold get_succ, has_arc, Env.MapsTo.
+  split; [intros H|intros (?&Hs&Hin)]; destruct Env.find.
+  3,4:inv Hs; auto.
+  - eauto.
+  - destruct (not_In_empty _ H).
+Qed.
+
+(** Get the predecessors of a vertex *)
+Definition get_pred (x : ident) (a : A_set) :=
+  Env.fold (fun y s acc => if PS.mem x s then (PS.add y acc) else acc) a PS.empty.
+
+Lemma get_pred_spec : forall a x y,
+    PS.In x (get_pred y a) <->
+    has_arc a x y.
+Proof.
+  intros *.
+  unfold get_pred, has_arc, Env.MapsTo.
+  apply Env.Props.P.fold_rec.
+  - intros ? Hempty.
+    rewrite Env.Empty_alt in Hempty.
+    split; [intros H|intros (?&Hfind&_)].
+    + destruct (not_In_empty _ H).
+    + rewrite Hempty in Hfind. congruence.
+  - intros * Hm Hnin Hadd Hrec.
+    rewrite Hadd; clear Hadd.
+    split; [intros H|intros (?&?&?)];
+      destruct (PS.mem _ _) eqn:Hmem; destruct (ident_eq_dec x k); subst.
+    + rewrite Env.gss; eauto.
+    + rewrite Env.gso; eauto.
+      apply PSF.add_3 in H; auto.
+      apply Hrec in H as (?&?&?); eauto.
+    + exfalso. apply Hrec in H as (?&Hfind&?).
+      apply Env.find_In in Hfind; auto.
+    + rewrite Env.gso; eauto.
+      apply Hrec in H as (?&?&?); eauto.
+    + apply PSF.add_1; auto.
+    + rewrite Env.gso in H; auto.
+      apply PSF.add_2. rewrite Hrec; eauto.
+    + exfalso.
+      rewrite Env.gss in H; auto. inv H.
+      apply PSE.mem_4 in Hmem; auto.
+    + rewrite Env.gso in H; auto.
+      rewrite Hrec; eauto.
+Qed.
+
+Definition has_trans_arc a := clos_trans_n1 _ (has_arc a).
+Hint Constructors clos_trans_n1.
+Hint Unfold has_trans_arc.
+
+Global Instance has_trans_arc_Transitive : forall a,
+    Transitive (has_trans_arc a).
+Proof.
+  intros ? ??? Ha1 Ha2.
+  induction Ha2; eauto.
+Qed.
+
+Lemma nhas_trans_arc_empty : forall x y,
+    ~has_trans_arc empty_arc_set x y.
+Proof.
+  intros * contra.
+  induction contra; eapply nhas_arc_empty; eauto.
+Qed.
+
+Fact add_arc_has_trans_arc1 : forall a x y,
+    has_trans_arc (add_arc x y a) x y.
+Proof.
+  left.
+  rewrite add_arc_spec; auto.
+Qed.
+
+Fact add_arc_has_trans_arc2 : forall a x y x' y',
+    has_trans_arc a x' y' ->
+    has_trans_arc (add_arc x y a) x' y'.
+Proof.
+  intros * Ha.
+  induction Ha.
+  - left. rewrite add_arc_spec; auto.
+  - eapply tn1_trans; eauto.
+    rewrite add_arc_spec; eauto.
+Qed.
+Hint Resolve add_arc_has_trans_arc1 add_arc_has_trans_arc2.
+
+Lemma add_arc_spec2 : forall a x y x' y',
+    has_trans_arc (add_arc x y a) x' y' <->
+    has_trans_arc a x' y' \/
+    (x = x' /\ y = y') \/
+    (x = x' /\ has_trans_arc a y y') \/
+    (has_trans_arc a x' x /\ y = y') \/
+    (has_trans_arc a x' x /\ has_trans_arc a y y').
+Proof.
+  intros *; split; intros Ha.
+  - induction Ha; try rewrite add_arc_spec in *.
+    + destruct H as [?|(?&?)]; subst; auto.
+    + destruct H as [?|(?&?)];
+        destruct IHHa as [?|[(?&?)|[(?&?)|[(?&?)|(?&?)]]]];
+        subst; eauto 10.
+  - destruct Ha as [?|[(?&?)|[(?&?)|[(?&?)|(?&?)]]]]; subst; eauto.
+    + etransitivity; eauto.
+    + etransitivity; eauto.
+    + etransitivity; eauto.
+      etransitivity; eauto.
+Qed.
+
+(** ** Acyclic graph *)
+
+(** Transitive, Directed Acyclic Graph *)
+Inductive AcyGraph : V_set -> A_set -> Prop :=
+| AGempty : AcyGraph PS.empty empty_arc_set
+| AGaddv : forall v a x,
+    AcyGraph v a ->
+    (* ~PS.In x v -> *)
+    AcyGraph (PS.add x v) a
+| AGadda : forall v a x y,
+    AcyGraph v a ->
+    x <> y ->
+    PS.In x v ->
+    PS.In y v ->
+    (* ~has_arc a x y -> *)
+    ~has_trans_arc a y x ->
+    AcyGraph v (add_arc x y a).
+Hint Constructors AcyGraph.
+
+Definition vertices {v a} (g : AcyGraph v a) : V_set := v.
+Definition arcs {v a} (g : AcyGraph v a) : A_set := a.
+
+Definition is_vertex {v a} (g : AcyGraph v a) (x : ident) : Prop :=
+  PS.In x v.
+
+Lemma is_vertex_spec {v a} : forall (g : AcyGraph v a) x,
+    is_vertex g x <-> PS.In x (vertices g).
+Proof. reflexivity. Qed.
+
+Definition is_arc {v a} (g : AcyGraph v a) x y : Prop :=
+  has_arc a x y.
+
+Lemma is_arc_spec {v a} : forall (g : AcyGraph v a) x y,
+    is_arc g x y <-> (has_arc (arcs g) x y).
+Proof. reflexivity. Qed.
+
+Lemma nis_arc_Gempty : forall x y,
+  ~is_arc AGempty x y.
+Proof.
+  intros * (?&contra&_).
+  rewrite Env.Props.P.F.empty_mapsto_iff in contra; auto.
+Qed.
+
+Definition is_trans_arc {v a} (g : AcyGraph v a) x y : Prop :=
+  has_trans_arc a x y.
+
+Lemma nis_trans_arc_Gempty : forall x y,
+    ~is_trans_arc AGempty x y.
+Proof.
+  intros * contra; simpl in contra.
+  apply nhas_trans_arc_empty in contra; auto.
+Qed.
+
+(** ** Major properties of is_arc : transitivity, irreflexivity, asymmetry *)
+
+Lemma has_arc_trans : forall a x y z,
+    has_arc a x y ->
+    has_arc a y z ->
+    has_trans_arc a x z.
+Proof.
+  intros * Ha1 Ha2; eauto.
+Qed.
+
+Global Instance is_trans_arc_Transitive {v a} (g : AcyGraph v a) :
+    Transitive (is_trans_arc g).
+Proof. eapply has_trans_arc_Transitive; eauto. Qed.
+
+Lemma has_arc_irrefl : forall v a,
+    AcyGraph v a ->
+    Irreflexive (has_arc a).
+Proof.
+  fix irrefl 3.
+  intros * g. destruct g.
+  - intros ? Ha.
+    apply nis_arc_Gempty in Ha; auto.
+  - specialize (irrefl _ _ g); auto.
+  - specialize (irrefl _ _ g).
+    intros x' Harc.
+    apply add_arc_spec in Harc as [?|(?&?)]; subst.
+    + eapply irrefl; eauto.
+    + congruence.
+Qed.
+
+Global Instance is_arc_Irreflexive {v a} (g : AcyGraph v a) :
+    Irreflexive (is_arc g).
+Proof. eapply has_arc_irrefl; eauto. Qed.
+
+Global Instance is_trans_arc_Asymmetric {v a} (g : AcyGraph v a) :
+    Asymmetric (is_trans_arc g).
+Proof.
+  revert v a g.
+  fix trans 3.
+  intros *. destruct g.
+  - intros ? ? ? Ha1.
+    exfalso. eapply nhas_trans_arc_empty; eauto.
+  - specialize (trans _ _ g); auto.
+  - specialize (trans _ _ g).
+    intros x' y' Harc1 Harc2.
+    apply add_arc_spec2 in Harc1; apply add_arc_spec2 in Harc2.
+    destruct Harc1 as [?|[(?&?)|[(?&?)|[(?&?)|(?&?)]]]];
+      destruct Harc2 as [?|[(?&?)|[(?&?)|[(?&?)|(?&?)]]]]; subst; eauto 10.
+    1-7:eapply n0.
+    1-7:etransitivity; eauto.
+    1,2:etransitivity; eauto.
+Qed.
+
+Corollary has_arc_asym : forall v a,
+    AcyGraph v a ->
+    Asymmetric (has_arc a).
+Proof.
+  intros * g ?? Ha1 Ha2.
+  eapply is_trans_arc_Asymmetric with (g0:=g); unfold is_trans_arc; eauto.
+Qed.
+
+Global Instance is_arc_Asymmetric {v a} (g : AcyGraph v a) :
+    Asymmetric (is_arc g).
+Proof. eapply has_arc_asym; eauto. Qed.
+
+Global Instance is_trans_arc_Irreflexive {v a} (g : AcyGraph v a) :
+  Irreflexive (is_trans_arc g).
+Proof.
+  revert v a g.
+  fix irrefl 3.
+  intros * x. destruct g.
+  - apply nis_trans_arc_Gempty.
+  - eapply (irrefl _ _ g).
+  - intros contra.
+    specialize (irrefl _ _ g).
+    apply add_arc_spec2 in contra as [?|[(?&?)|[(?&?)|[(?&?)|(?&?)]]]]; subst; eauto.
+    + eapply irrefl; eauto.
+    + eapply n0. etransitivity; eauto.
+Qed.
+
+Definition is_arcb {v a} (g : AcyGraph v a) x y : bool :=
+  has_arcb a x y.
+
+Lemma is_arcb_spec {v a} : forall (g : AcyGraph v a) x y,
+    is_arcb g x y = true <-> is_arc g x y.
+Proof.
+  intros *.
+  unfold is_arcb. rewrite has_arcb_spec.
+  reflexivity.
+Qed.
+
+Corollary is_arcb_false_iff {v a} : forall (g : AcyGraph v a) x y,
+    is_arcb g x y = false <-> ~is_arc g x y.
+Proof.
+  intros *.
+  rewrite <- is_arcb_spec, Bool.not_true_iff_false.
+  reflexivity.
+Qed.
+
+Lemma is_arc_is_vertex : forall {v a} (g : AcyGraph v a) x y,
+    is_arc g x y ->
+    is_vertex g x /\ is_vertex g y.
+Proof.
+  fix is_arc_is_vertex 3.
+  intros * Hisarc.
+  destruct g; simpl in *.
+  - exfalso. destruct Hisarc as (?&contra&_).
+    rewrite Env.Props.P.F.empty_mapsto_iff in contra; auto.
+  - specialize (is_arc_is_vertex _ _ g).
+    apply is_arc_is_vertex in Hisarc as (Hvx&Hvy).
+    split; apply PSF.add_2; auto.
+  - specialize (is_arc_is_vertex _ _ g).
+    unfold is_arc in Hisarc.
+    apply add_arc_spec in Hisarc as [?|(?&?)]; subst; auto.
+    apply is_arc_is_vertex in H; auto.
+Qed.
+
+Corollary is_trans_arc_is_vertex : forall {v a} (g : AcyGraph v a) x y,
+    is_trans_arc g x y ->
+    is_vertex g x /\ is_vertex g y.
+Proof.
+  intros * Ha.
+  induction Ha.
+  - apply is_arc_is_vertex; auto.
+  - destruct IHHa.
+    eapply is_arc_is_vertex in H as (_&?).
+    eauto.
+Qed.
+
+Lemma is_trans_arc_neq : forall {v a} (g : AcyGraph v a) x y,
+    is_trans_arc g x y ->
+    x <> y.
+Proof.
+  intros * Ha contra; subst.
+  eapply is_trans_arc_Irreflexive; eauto.
+Qed.
+
+(** has_arc is decidable ! *)
+Lemma has_arc_dec : forall a,
+    forall x y, (has_arc a x y) \/ (~has_arc a x y).
+Proof.
+  intros *.
+  unfold has_arc.
+  destruct (Env.find x a) eqn:Hfind.
+  - destruct (PS.mem y t) eqn:Hmem; [left|right].
+    + apply PSF.mem_2 in Hmem.
+      exists t; split; auto.
+    + intros (?&Hmap&Hin).
+      unfold Env.MapsTo in *. rewrite Hfind in Hmap. inv Hmap.
+      apply PSF.mem_1 in Hin. congruence.
+  - right. intros (?&Hmap&_).
+    unfold Env.MapsTo in *. rewrite Hfind in Hmap. inv Hmap.
+Qed.
+
+Local Ltac destruct_conj_disj :=
+    match goal with
+    | H : _ /\ _ |- _ => destruct H
+    | H : _ \/ _ |- _ => destruct H
+    end; subst.
+
+(** is_trans_arc is decidable ! *)
+Lemma is_trans_arc_dec : forall {v a} (g : AcyGraph v a),
+    forall x y, (is_trans_arc g x y) \/ (~ is_trans_arc g x y).
+Proof.
+  fix is_trans_arc_dec 3.
+  intros *. destruct g.
+  - right. eapply nis_trans_arc_Gempty.
+  - specialize (is_trans_arc_dec _ _ g x y) as [?|?]; auto.
+  - specialize (is_trans_arc_dec _ _ g).
+    destruct (is_trans_arc_dec x y), (is_trans_arc_dec x x0), (is_trans_arc_dec y0 y),
+    (ident_eq_dec y y0), (ident_eq_dec x x0); subst.
+    1-32: try solve [left; apply add_arc_spec2; auto 10].
+    1-7:(right; intro contra; apply add_arc_spec2 in contra;
+         repeat destruct_conj_disj; auto).
+Qed.
+
+(** ** Building an acyclic graph
+    We can try to build an acyclic graph from any graph
+    (defined as a mapping from vertices to their direct predecessors)
+    We iterate through the list of vertices, trying to add some that are
+    not already in the graph, and which predecessors are all already in the graph *)
+
+From compcert Require Import common.Errors.
+
+Definition add_after (preds : PS.t) (x : ident) (a : A_set) : A_set :=
+  PS.fold (fun p a => add_arc p x a) preds a.
+
+Lemma add_after_spec : forall a preds y x' y',
+    has_arc (add_after preds y a) x' y' <->
+    has_arc a x' y' \/
+    (PS.In x' preds /\ y = y').
+Proof.
+  Local Ltac simpl_ps_add :=
+    unfold PSP.Add in *;
+    match goal with
+    | Hadd: (forall y, PS.In y ?s2 <-> ?p = y \/ PS.In y ?s1), Hin: PS.In ?x ?s1 |- _ =>
+      eapply or_intror in Hin; erewrite <- Hadd in Hin
+    | Hadd: (forall y, PS.In y ?s2 <-> ?x = y \/ PS.In y ?s1) |- _ =>
+      specialize (Hadd x) as (_&?)
+    | _ => idtac
+  end.
+  intros preds a y.
+  unfold add_after. apply PSP.fold_rec.
+  - intros * Hemp.
+    split; auto.
+    intros [?|(Hin&?)]; subst; auto.
+    destruct (Hemp _ Hin).
+  - intros p * Hin Hnin Hadd Hrec *.
+    rewrite add_arc_spec.
+    split; intros [?|(?&?)]; subst; auto.
+    + apply Hrec in H as [?|(?&?)]; subst; auto; unfold PS.Exists.
+      repeat simpl_ps_add; eauto 10.
+    + repeat simpl_ps_add; eauto 10.
+    + rewrite Hrec; auto.
+    + destruct (ident_eq_dec p x'); subst; auto.
+      specialize (Hrec x' y').
+      left. rewrite Hrec; auto.
+      right. split; auto.
+      apply Hadd in H as [?|?]; auto. congruence.
+Qed.
+
+Corollary add_after_has_arc1 : forall a x y x' preds,
+    has_arc a x y ->
+    has_arc (add_after preds x' a) x y.
+Proof.
+  intros * Ha.
+  rewrite add_after_spec; auto.
+Qed.
+
+Corollary add_after_has_arc2 : forall a x y preds,
+    PS.In y preds ->
+    has_arc (add_after preds x a) y x.
+Proof.
+  intros * Hin.
+  rewrite add_after_spec; auto.
+Qed.
+
+Fact add_after_has_trans_arc2 : forall a preds y x' y',
+    has_trans_arc a x' y' ->
+    has_trans_arc (add_after preds y a) x' y'.
+Proof.
+  intros * Ha.
+  induction Ha.
+  - left. rewrite add_after_spec; auto.
+  - eapply tn1_trans; eauto. rewrite add_after_spec; auto.
+Qed.
+
+Lemma add_after_spec2 : forall a preds y x' y',
+    has_trans_arc (add_after preds y a) x' y' <->
+    has_trans_arc a x' y' \/
+    (PS.In x' preds /\ y = y') \/
+    (PS.In x' preds /\ has_trans_arc a y y') \/
+    (PS.Exists (fun p => has_trans_arc a x' p) preds /\ y = y') \/
+    (PS.Exists (fun p => has_trans_arc a x' p) preds /\ has_trans_arc a y y').
+Proof.
+  intros *; split; intros Ha.
+  - induction Ha; rewrite add_after_spec in *.
+    + destruct H as [?|(?&?)]; subst; auto.
+    + destruct H as [?|(?&?)];
+        destruct IHHa as [?|[(?&?)|[(?&?)|[(?&?)|(?&?)]]]];
+        subst; eauto 10.
+      do 3 right. left. split; auto.
+      eexists; eauto.
+  - destruct Ha as [?|[(?&?)|[(?&?)|[(?&?)|(?&?)]]]]; subst; eauto.
+    + eapply add_after_has_trans_arc2; eauto.
+    + left. rewrite add_after_spec; auto.
+    + eapply add_after_has_trans_arc2 in H0.
+      etransitivity; eauto.
+      left. rewrite add_after_spec; eauto.
+    + destruct H as (?&Hin&Ha).
+      eapply add_after_has_trans_arc2 in Ha.
+      etransitivity; eauto.
+      left. rewrite add_after_spec; eauto.
+    + destruct H as (?&Hin&Ha).
+      eapply add_after_has_trans_arc2 in Ha.
+      eapply add_after_has_trans_arc2 in H0.
+      etransitivity; eauto.
+      etransitivity; eauto.
+      left. rewrite add_after_spec; eauto.
+Qed.
+
+Corollary add_after_has_trans_arc1 : forall a preds x' y',
+    PS.In x' preds ->
+    has_trans_arc (add_after preds y' a) x' y'.
+Proof.
+  intros * Hin.
+  rewrite add_after_spec2; auto.
+Qed.
+
+Corollary add_after_has_trans_arc3 : forall {v a} x y preds,
+    AcyGraph v a ->
+    ~PS.In y v ->
+    has_trans_arc (add_after preds y a) x y ->
+    PS.In x preds \/ PS.Exists (fun x' => has_trans_arc a x x') preds.
+Proof.
+  intros * Hacy Hnin Ha.
+  rewrite add_after_spec2 in Ha.
+  repeat destruct_conj_disj; auto.
+  exfalso.
+  eapply is_trans_arc_is_vertex with (g:=Hacy) in H as (?&?); eauto.
+Qed.
+
+Lemma add_after_AcyGraph : forall v a x preds,
+    PS.In x v ->
+    ~PS.In x preds ->
+    PS.For_all (fun x => PS.In x v) preds ->
+    PS.For_all (fun p => ~has_trans_arc a x p) preds ->
+    AcyGraph v a ->
+    AcyGraph v (add_after preds x a) /\
+    PS.For_all (fun p => ~has_trans_arc (add_after preds x a) x p) preds.
+Proof.
+  intros * Hin1 Hnin2 Hpreds Hna Hacy.
+  revert Hacy.
+  unfold add_after. eapply PSP.fold_rec_nodep.
+  - intros * Hacy; split; auto.
+  - intros * Hin' Hrec Hacy.
+    specialize (Hrec Hacy) as (Hacy'&Hna').
+    split; [apply AGadda|]; auto.
+    + intro contra; subst; auto.
+    + intros ? Hin contra.
+      apply Hna' in Hin. apply Hin.
+      rewrite add_arc_spec2 in contra. repeat destruct_conj_disj; auto.
+      * exfalso; auto.
+      * exfalso; auto.
+        apply Hna' in Hin'; auto.
+Qed.
+
+Corollary add_after_AcyGraph' : forall v a x preds,
+    ~PS.In x v ->
+    ~PS.In x preds ->
+    PS.For_all (fun x => PS.In x v) preds ->
+    AcyGraph v a ->
+    AcyGraph (PS.add x v) (add_after preds x a).
+Proof.
+  intros * Hnin1 Hnin2 Hpreds Hacy.
+  assert (PS.For_all (fun y => ~has_trans_arc a x y) preds) as Hnpreds.
+  { intros ? Hin contra.
+    specialize (is_trans_arc_is_vertex Hacy) as (?&?); eauto.
+  }
+  eapply add_after_AcyGraph; eauto.
+  - apply PSF.add_1; auto.
+  - intros ? Hin. apply Hpreds in Hin.
+    apply PSF.add_2; auto.
+Qed.
+
+Definition find_addable (v : V_set) (g : Env.t PS.t) :=
+  Env.find_pred (fun k preds =>
+                   andb (negb (PS.mem k v))
+                        (PS.for_all (fun x => PS.mem x v) preds)) g.
+
+Definition errmsg_of_env {A} (s : Env.t A) :=
+  Env.fold (fun x _ a => (CTX x)::(MSG ", ")::a) s nil.
+
+Definition acgraph_of_graph g v a :=
+  (forall x, Env.In x g <-> PS.In x v) /\
+  (forall x y, (exists xs, Env.find y g = Some xs /\ PS.In x xs) -> has_arc a x y).
+
+Program Fixpoint bacg_aux
+        (g0 g : Env.t PS.t)
+        (Href : Env.refines eq g g0)
+        v (ag : exists a, AcyGraph v a /\ acgraph_of_graph (Env.diff g0 g) v a) {measure (Env.cardinal g)}
+  : res { v | exists a, AcyGraph v a /\ acgraph_of_graph g0 v a } :=
+  match Env.is_empty g with
+    | true => OK (exist _ v _)
+    | false =>
+      match (find_addable v g) with
+      | None => Error (MSG "Cannot build acyclic graph, there is a cycle between the following vars : "::(errmsg_of_env g))
+      | Some (x, preds) => bacg_aux g0 (Env.remove x g) _ (PS.add x v) _
+      end
+  end.
+Next Obligation.
+  exists ag. split; auto.
+  rename Heq_anonymous into Hempty. symmetry in Hempty.
+  apply Env.is_empty_2 in Hempty.
+  clear bacg_aux. destruct H0 as (Hv&Ha).
+  constructor.
+  - intros ?.
+    rewrite <- Hv.
+    rewrite Env.diff_empty; auto. reflexivity.
+  - intros * (?&Hfind&?).
+    apply Ha. eexists; split; eauto.
+    rewrite Env.diff_empty; auto.
+Qed.
+Next Obligation.
+  etransitivity; [|eauto].
+  eapply Env.refines_remove; auto.
+Qed.
+Next Obligation.
+  clear bacg_aux.
+  rename Heq_anonymous into Hfind. symmetry in Hfind.
+  rename Heq_anonymous0 into Hempty. symmetry in Hempty.
+  apply Env.find_pred_spec in Hfind as (Hin&Hb).
+  apply Bool.andb_true_iff in Hb as (Hnin&Hpreds).
+  apply Bool.negb_true_iff, PSE.mem_4 in Hnin.
+  rewrite PS.for_all_spec in Hpreds. 2:intros ? ? Heq; rewrite Heq; auto.
+  exists (add_after preds x ag). destruct H0 as (Hv&Ha).
+  split; [|split].
+  - eapply add_after_AcyGraph'; eauto.
+    intro contra. apply Hpreds in contra; auto.
+  - intros ?.
+    rewrite PS.add_spec, <- Hv.
+    repeat rewrite Env.diff_In_iff.
+    split; [intros (?&Hnin')|intros [?|(?&Hnin')]]; subst.
+    + destruct (ident_eq_dec x0 x); auto.
+      right; split; auto.
+      intros contra. apply Hnin'.
+      rewrite Env.Props.P.F.remove_in_iff; auto.
+    + split.
+      * exists preds. eapply Href in Hin as (?&Heq&?); subst; auto.
+      * apply Env.remove_1. reflexivity.
+    + split; auto.
+      intro contra. apply Hnin'.
+      apply Env.Props.P.F.remove_in_iff in contra as (?&?); auto.
+  - intros x' y' (?&Hfind&Hin').
+    specialize (Ha x' y').
+    assert (Hfind':=Hfind). apply Env.diff_remove in Hfind' as [(Hneq&Hfind')|?]; subst.
+    + specialize (Ha (ex_intro _ _ (conj Hfind' Hin'))) as Harc.
+      apply add_after_has_arc1; auto.
+    + apply Env.diff_spec in Hfind as (Hfind&?).
+      apply Href in Hin as (?&?&Hin); subst.
+      rewrite Hfind in Hin. inv Hin.
+      apply add_after_has_arc2; auto.
+Qed.
+Next Obligation.
+  clear Heq_anonymous0.
+  rename Heq_anonymous into Hfind. symmetry in Hfind.
+  apply Env.find_pred_spec in Hfind as (Hin&_).
+  erewrite (@Env.Props.P.cardinal_2 _ _ g).
+  - apply PeanoNat.Nat.lt_succ_diag_r.
+  - apply Env.remove_1. reflexivity.
+  - unfold Env.Props.P.Add. intros ?.
+    rewrite <- Env.add_remove; auto. apply Hin.
+Qed.
+
+Program Definition build_acyclic_graph (g : Env.t PS.t) : res { v | exists a, AcyGraph v a /\ acgraph_of_graph g v a } :=
+  bacg_aux g g _ PS.empty _.
+Next Obligation.
+  exists empty_arc_set; split; auto.
+  split.
+  - intros ?.
+    split; intros H; exfalso.
+    + apply Env.In_find in H as (?&Hfind).
+      apply Env.diff_spec in Hfind as (Hmap&Hnin).
+      apply Env.find_In in Hmap; auto.
+    + apply not_In_empty in H; auto.
+  - intros xs ? (?&Hfind&Hin).
+    exfalso.
+    apply Env.diff_spec in Hfind as (Hmap&Hnin).
+    apply Env.find_In in Hmap; auto.
+Qed.
+
+(** ** Extracting a prefix
+    In order to build an induction principle over the graph, we need to linearize it.
+    We want to extract a "prefix" from the graph, which is an order of the vertices
+    in which arcs are directed from the tail of the list to the head
+ *)
+
+Definition Prefix {v a} (g : AcyGraph v a) (xs : list ident) :=
+  ForallTail (fun x xs => ~In x xs /\ is_vertex g x /\ (forall y, is_trans_arc g y x -> In y xs)) xs.
+Hint Unfold Prefix.
+
+Lemma Prefix_weaken : forall {v a} (g : AcyGraph v a) xs,
+    Prefix g xs ->
+    Forall (fun x => forall y, is_trans_arc g y x -> In y xs) xs.
+Proof.
+  intros * Hpref.
+  induction Hpref; auto.
+  destruct H as (Hnin&Hv&Ha).
+  constructor; intuition.
+  eapply Forall_impl; [|eauto].
+  intros * ? ? ?. right; auto.
+Qed.
+
+Lemma Prefix_nIn : forall {v a} (g : AcyGraph v a) x xs,
+    ~In x xs ->
+    Prefix g xs ->
+    ~Exists (fun y => is_trans_arc g x y) xs.
+Proof.
+  intros * Hnin Hpre Hex.
+  apply Prefix_weaken in Hpre.
+  eapply Forall_Exists in Hex; eauto.
+  eapply Exists_exists in Hex as (?&_&Ha&Ha').
+  specialize (Ha _ Ha'); auto.
+Qed.
+
+Lemma Prefix_NoDup : forall {v a} (g : AcyGraph v a) xs,
+    Prefix g xs ->
+    NoDup xs.
+Proof.
+  intros * Hpref.
+  induction Hpref; constructor; auto.
+  destruct H; auto.
+Qed.
+
+Fact Prefix_AGaddv : forall {v a} (g : AcyGraph v a) x xs,
+    Prefix g xs ->
+    Prefix (AGaddv v a x g) xs.
+Proof.
+  induction xs; intros * Hpre; inv Hpre; auto.
+  destruct H1 as (?&?&?).
+  specialize (IHxs H2).
+  repeat constructor; auto.
+  apply PSF.add_2; auto.
+Qed.
+
+Lemma Prefix_insert : forall {v a} (g : AcyGraph v a) xs1 xs2 x,
+    is_vertex g x ->
+    ~In x (xs1++xs2) ->
+    (forall y, is_trans_arc g y x -> In y xs2) ->
+    Prefix g (xs1 ++ xs2) ->
+    Prefix g (xs1 ++ x :: xs2).
+Proof.
+  induction xs1; intros * Hver Hnin Ha Hpre; simpl in *.
+  - constructor; repeat split; auto.
+  - inversion_clear Hpre as [|?? (Hnin'&Hver'&Ha') Hpre'].
+    apply not_or' in Hnin as (Hneq&Hnin).
+    apply not_In_app in Hnin' as (Hnin1&Hnin2).
+    constructor; repeat split; auto.
+    + rewrite not_In_app; simpl; rewrite not_or'; auto.
+    + intros * Ha''. specialize (Ha' _ Ha'').
+      rewrite in_app_iff in *; simpl.
+      destruct Ha'; auto.
+    + apply IHxs1; auto.
+Qed.
+
+(** x is located before y in l *)
+Definition Before (x y : ident) l :=
+  ForallTail (fun x' xs => x' = y -> In x xs) l.
+
+Lemma Before_middle : forall xs1 xs2 x y,
+    x <> y ->
+    ~In y xs1 ->
+    ~In y xs2 ->
+    Before x y (xs1 ++ y :: x :: xs2).
+Proof.
+  induction xs1; intros * Hneq Hnin1 Hnin2; simpl.
+  - constructor; [|constructor].
+    + intros _. left; auto.
+    + intros contra; subst. congruence.
+    + induction xs2; auto.
+      apply not_in_cons in Hnin2 as (Hneq'&Hnin2).
+      constructor; auto.
+      intros contra; subst. congruence.
+  - apply not_in_cons in Hnin1 as (Hneq'&Hnin1).
+    constructor; auto.
+    + intros contra; subst. congruence.
+    + apply IHxs1; auto.
+Qed.
+
+Lemma Before_In : forall xs x y,
+    Before x y xs ->
+    In y xs ->
+    In x xs.
+Proof.
+  induction xs; intros * Hbef Hin; inv Hbef; inv Hin.
+  1,2:right; eauto.
+Qed.
+
+Import Permutation.
+
+(** Given a prefix of the form xs1 ++ y :: xs2, we can split xs1
+    into two list: xs1l depends on y and xs1r doesnt *)
+Fact Prefix_Partition_split : forall {v a} (g : AcyGraph v a) xs1 xs2 xs1l xs1r y,
+    Partition (fun z => is_trans_arc g y z) xs1 xs1l xs1r ->
+    Prefix g (xs1 ++ y :: xs2) ->
+    Prefix g (xs1l ++ y :: xs1r ++ xs2).
+Proof.
+  induction xs1; intros * Hpart Hpre; inv Hpart; simpl in *.
+  - assumption.
+  - inversion_clear Hpre as [|?? (Hnin&Hver&Ha) Hf].
+    constructor; repeat split; auto.
+    + erewrite (Partition_Permutation _ xs1), <- app_assoc, <- Permutation_middle in Hnin; eauto.
+    + intros * Ha'. specialize (Ha _ Ha').
+      erewrite (Partition_Permutation _ xs1), <- app_assoc, <- Permutation_middle in Ha; eauto.
+    + apply IHxs1; auto.
+  - inversion_clear Hpre as [|?? (Hnin&Hver&Ha) Hf].
+    rewrite cons_is_app, app_assoc.
+    apply Prefix_insert; auto; try rewrite <- app_assoc, <- cons_is_app.
+    + erewrite (Partition_Permutation _ xs1), <- app_assoc, <- Permutation_middle in Hnin; eauto.
+    + intros * Ha'. specialize (Ha _ Ha').
+      erewrite (Partition_Permutation _ xs1), <- app_assoc in Ha; eauto.
+      repeat (rewrite in_app_iff in *; simpl in *; idtac).
+      destruct Ha as [Hin|[?|[?|?]]]; subst; auto. 2:congruence.
+      exfalso.
+      eapply Partition_Forall1, Forall_forall in H1; [|eauto].
+      eapply H4; eauto. etransitivity; eauto.
+    + apply IHxs1; auto.
+Qed.
+
+(* Is there is no arc between y and x, it is possible to reorganize the Prefix *)
+(* so that x ends up before y *)
+Lemma Prefix_reorganize : forall {v a} (g : AcyGraph v a) xs x y,
+    x <> y ->
+    In x xs ->
+    In y xs ->
+    Prefix g xs ->
+    ~is_trans_arc g y x ->
+    exists xs', Permutation.Permutation xs' xs /\
+           Prefix g xs' /\
+           Before x y xs'.
+Proof.
+  induction xs; intros * Hneq Hin1 Hin2 Hpref Hna;
+    inv Hin1; inv Hin2; inversion_clear Hpref as [|?? (Hnin&Hv&Ha)]; subst.
+  - contradiction.
+  - clear IHxs.
+    apply in_split in H as (xs1&xs2&?); subst.
+    (* Partition the xs1.
+       No xs1 depends on x (because (xs1 ++ y :: xs2) is a prefix).
+       All the xs1l depend on y, and therefore x does not depend on them.
+       All the xs1r do not depend on y
+       We produce a new list of the form xs1l ++ y :: x :: xs1r ++ xs2
+     *)
+    assert (exists xs1l xs1r, Partition (fun z => is_trans_arc g y z) xs1 xs1l xs1r) as (xs1l&xs1r&Hpart).
+    { eapply dec_Partition, is_trans_arc_dec. }
+    exists (xs1l ++ y :: x :: xs1r ++ xs2).
+    assert (Permutation xs1 (xs1l ++ xs1r)) as Hperm.
+    { eapply Partition_Permutation; eauto. }
+    repeat split.
+    + repeat rewrite <- Permutation_middle.
+      rewrite app_assoc, <- Hperm.
+      apply perm_swap.
+    + eapply Prefix_Partition_split in H0; eauto.
+      rewrite cons_is_app, app_assoc.
+      apply Prefix_insert; try rewrite <- app_assoc, <- cons_is_app; auto.
+      * rewrite Hperm, <- app_assoc, <- Permutation_middle in Hnin; auto.
+      * intros ? Ha'. specialize (Ha _ Ha').
+        rewrite Hperm, <- app_assoc in Ha.
+        repeat (rewrite in_app_iff in *; simpl in *; idtac).
+        destruct Ha as [?|[?|[?|?]]]; subst; auto. 2:congruence.
+        exfalso.
+        eapply Partition_Forall1, Forall_forall in Hpart; [|eauto].
+        eapply Hna. etransitivity; eauto.
+    + assert (~ In y (xs1 ++ xs2)).
+      { apply Prefix_NoDup in H0.
+        rewrite <- Permutation_middle in H0.
+        inv H0; auto. }
+      rewrite Hperm, <- app_assoc in H.
+      apply not_In_app in H as (?&?).
+      apply Before_middle; auto.
+  - exists (y::xs). repeat split; auto.
+    constructor; auto.
+    clear - Hnin.
+    induction xs; [constructor|].
+    apply not_in_cons in Hnin as (Hneq&Hnin).
+    constructor; eauto.
+    intro contra; subst; congruence.
+  - specialize (IHxs _ _ Hneq H H0 H1 Hna) as (xs'&Hperm&Hpre&Hbef).
+    exists (a0::xs'); repeat split; auto.
+    + repeat constructor; auto.
+      2:intros ? Ha'.
+      1,2:rewrite Hperm; auto.
+    + constructor; auto.
+      intros ?; subst.
+      rewrite Hperm; auto.
+Qed.
+
+Lemma Prefix_AGadda : forall {v a} (g : AcyGraph v a) xs x y Hneq Hin1 Hin2 Hna,
+    Before x y xs ->
+    Prefix g xs ->
+    Prefix (AGadda _ _ x y g Hneq Hin1 Hin2 Hna) xs.
+Proof.
+  induction xs; intros * Hbef Hpre; auto.
+  inv Hbef. inversion_clear Hpre as [|?? (?&?&?) Hf].
+  constructor. 2:eapply IHxs; eauto.
+  repeat split; auto.
+  intros ? Ha.
+  apply add_arc_spec2 in Ha as [?|[(?&?)|[(?&?)|[(?&?)|(?&?)]]]]; subst; auto.
+  - apply H3 in H5; auto.
+    eapply Before_In in H2; eauto.
+  - specialize (H1 eq_refl).
+    eapply Prefix_weaken, Forall_forall in Hf; eauto.
+  - specialize (H3 _ H5).
+    eapply Before_In in H2; eauto.
+    eapply Prefix_weaken, Forall_forall in Hf; eauto.
+Qed.
+
+(** Every Directed Acyclic Graph has at least one complete Prefix *)
+Lemma has_Prefix : forall {v a} (g : AcyGraph v a),
+    exists xs, (PS.Equal (vertices g) (PSP.of_list xs)) /\
+          Prefix g xs.
+Proof.
+  fix has_Prefix 3.
+  intros *.
+  destruct g.
+  - exists []; simpl. split; auto.
+    reflexivity.
+  - specialize (has_Prefix _ _ g) as (xs&Heq&Hp).
+    destruct (PSP.In_dec x v).
+    + exists xs; simpl; split; auto.
+      * rewrite <- Heq.
+        intros ?. setoid_rewrite PSF.add_iff.
+        split; [intros [?|?]| intros ?]; subst; auto.
+      * apply Prefix_AGaddv; auto.
+    + exists (x::xs); simpl; split; [|constructor;repeat split].
+      * unfold vertices in *.
+        rewrite Heq. reflexivity.
+      * rewrite Heq, <- ps_from_list_ps_of_list, ps_from_list_In in n; auto.
+      * apply PSF.add_1; auto.
+      * intros y Hisarc.
+        assert (Hneq:=Hisarc). apply is_trans_arc_neq in Hneq.
+        apply is_trans_arc_is_vertex in Hisarc as (?&?).
+        apply PSF.add_3 in H; auto.
+        rewrite <- ps_from_list_ps_of_list in Heq.
+        rewrite <- ps_from_list_In, <- Heq; auto.
+      * apply Prefix_AGaddv; auto.
+  - specialize (has_Prefix _ _ g) as (xs&Heq&Hp).
+    specialize (Prefix_reorganize g xs x y) as (xs'&?&Hp'&Hbef); auto.
+    + rewrite Heq, <- ps_from_list_ps_of_list, ps_from_list_In in i; auto.
+    + rewrite Heq, <- ps_from_list_ps_of_list, ps_from_list_In in i0; auto.
+    + exists xs'; split.
+      * rewrite <- ps_from_list_ps_of_list, H, ps_from_list_ps_of_list.
+        assumption.
+      * eapply Prefix_AGadda; eauto.
+Qed.
+
+(** ** Inserting into the graph
+    When we compile the program, what we do is often add some intermediate vertices
+    between a set of predecessors and an existing vertex.
+ *)
+
+Definition add_between preds x y a :=
+  add_arc x y (add_after preds x a).
+
+Lemma add_between_AcyGraph : forall {v a} (g : AcyGraph v a) x preds succ,
+    PS.For_all (is_vertex g) preds ->
+    is_vertex g succ ->
+    PS.For_all (fun p => is_arc g p succ) preds ->
+    ~is_vertex g x ->
+    AcyGraph (PS.add x v) (add_between preds x succ a).
+Proof.
+  intros * Hv1 Hv2 Harcs Hnv.
+  unfold add_between.
+  assert (~has_trans_arc a succ x) as Hna.
+  { intro contra.
+    eapply is_trans_arc_is_vertex in contra as (?&?); eauto. }
+  apply AGadda. apply add_after_AcyGraph'; auto.
+  - intro contra; subst.
+    contradiction.
+  - apply PSF.add_1; auto.
+  - apply PSF.add_2; auto.
+  - intro contra.
+    apply add_after_spec2 in contra as [?|[(?&?)|[(?&?)|[(?&?)|(?&?)]]]]; subst; auto.
+    + eapply Harcs, has_arc_irrefl in H; eauto.
+    + eapply is_trans_arc_Irreflexive in H0; eauto.
+    + destruct H as (p&Hin&Ha). apply Harcs in Hin.
+      eapply is_trans_arc_Asymmetric with (g0:=g) in Ha.
+      eapply Ha. left; eauto.
+    + eapply is_trans_arc_Irreflexive in H0; eauto.
+Qed.
+
+Lemma add_between_spec : forall v a preds x y x' y',
+    ~PS.In y preds ->
+    ~PS.Exists (fun p => has_arc a y p) preds ->
+    AcyGraph v a ->
+    has_arc (add_between preds x y a) x' y' <->
+    has_arc a x' y' \/
+    PS.In x' preds /\ x = y' \/
+    x = x' /\ y = y'.
+Proof.
+  intros * Hnin1 Hnin2 Hg. unfold add_between.
+  rewrite add_arc_spec, add_after_spec.
+  split; intros; repeat destruct_conj_disj; eauto 10.
+Qed.
+
+Fact add_between_has_trans_arc2 : forall v a preds x y x' y',
+    ~PS.In y preds ->
+    ~PS.Exists (fun p => has_arc a y p) preds ->
+    AcyGraph v a ->
+    has_trans_arc a x' y' ->
+    has_trans_arc (add_between preds x y a) x' y'.
+Proof.
+  intros * Hnin1 Hnin2 Hg Ha.
+  induction Ha.
+  - left. rewrite add_between_spec; eauto.
+  - eapply tn1_trans; eauto. rewrite add_between_spec; eauto.
+Qed.
+
+Lemma add_between_spec2 : forall v a preds x y x' y',
+    ~PS.In y preds ->
+    ~PS.Exists (fun p => has_trans_arc a y p) preds ->
+    AcyGraph v a ->
+    has_trans_arc (add_between preds x y a) x' y' <->
+    has_trans_arc a x' y' \/
+    PS.In x' preds /\ x = y' \/
+    PS.In x' preds /\ y = y' \/
+    x = x' /\ y = y' \/
+    PS.Exists (fun p => has_trans_arc a x' p) preds /\ x = y' \/
+    PS.Exists (fun p => has_trans_arc a x' p) preds /\ y = y' \/
+    has_trans_arc a x' x /\ y = y' \/
+    PS.In x' preds /\ has_trans_arc a x y' \/
+    PS.In x' preds /\ has_trans_arc a y y' \/
+    x = x' /\ has_trans_arc a y y' \/
+    PS.Exists (fun p => has_trans_arc a x' p) preds /\ has_trans_arc a x y' \/
+    PS.Exists (fun p => has_trans_arc a x' p) preds /\ has_trans_arc a y y' \/
+    has_trans_arc a x' x /\ has_trans_arc a y y'.
+Proof.
+  intros * Hnin1 Hnin2 Hacy.
+  assert (~PS.Exists (fun p => has_arc a y p) preds) as Hnin3.
+  { intros (x0&Hin&contra).
+    apply Hnin2. exists x0; auto. }
+  split; intros; unfold PS.Exists in *.
+  - induction H.
+    + eapply add_between_spec in H; eauto.
+      repeat destruct_conj_disj; eauto 10.
+    + clear H0. eapply add_between_spec in H; eauto.
+      repeat destruct_conj_disj; eauto 16.
+      * exfalso; auto.
+      * exfalso; eauto.
+  - repeat destruct_conj_disj; eauto 15.
+    + eapply add_between_has_trans_arc2; eauto.
+    + left. rewrite add_between_spec; eauto.
+    + etransitivity. 2:apply add_arc_has_trans_arc1.
+      apply add_arc_has_trans_arc2.
+      rewrite add_after_spec2; auto.
+    + apply add_arc_has_trans_arc1.
+    + destruct H as (?&Hin&Ha).
+      etransitivity. eapply add_between_has_trans_arc2; eauto.
+      left; eapply add_between_spec; eauto.
+    + destruct H as (?&Hin&Ha).
+      etransitivity. eapply add_between_has_trans_arc2; eauto.
+      etransitivity; left; eapply add_between_spec; eauto.
+    + etransitivity. eapply add_between_has_trans_arc2; eauto.
+      left; eapply add_between_spec; eauto.
+    + etransitivity. 2:eapply add_between_has_trans_arc2; eauto.
+      left; eapply add_between_spec; eauto.
+    + etransitivity. 2:eapply add_between_has_trans_arc2; eauto.
+      etransitivity; left; eapply add_between_spec; eauto.
+    + etransitivity. 2:eapply add_between_has_trans_arc2; eauto.
+      left; eapply add_between_spec; eauto.
+    + destruct H as (?&Hin&Ha).
+      etransitivity. etransitivity. 1,3:eapply add_between_has_trans_arc2; eauto.
+      left; eapply add_between_spec; eauto.
+    + destruct H as (?&Hin&Ha).
+      etransitivity. etransitivity. 1,3:eapply add_between_has_trans_arc2; eauto.
+      etransitivity; left; eapply add_between_spec; eauto.
+    + etransitivity. etransitivity. 1,3:eapply add_between_has_trans_arc2; eauto.
+      left; eapply add_between_spec; eauto.
+Qed.
+
+Section remove_arc.
+
+  Definition remove_arc x y (a : A_set) : A_set :=
+    match (Env.find x a) with
+    | Some s => Env.add x (PS.remove y s) a
+    | None => a
+    end.
+
+  Lemma remove_arc_spec : forall a x y x' y' ,
+      has_arc (remove_arc x y a) x' y' <-> has_arc a x' y' /\ (x <> x' \/ y <> y').
+  Proof.
+    intros *. unfold remove_arc, has_arc, Env.MapsTo in *.
+    split; intros H;
+      [destruct H as (s&Hm&Hin)|destruct H as (?&?)];
+      destruct (ident_eq_dec x x'), (ident_eq_dec y y'), (Env.find x a) eqn:Hfind; subst.
+    1-16:try rewrite Env.gss in *; eauto.
+    1-16:try rewrite Env.gso in *; eauto.
+    - exfalso. inv Hm.
+      apply PSF.remove_1 in Hin; auto.
+    - congruence.
+    - split; auto.
+      inv Hm. exists t; split; auto.
+      apply PSF.remove_3 in Hin; auto.
+    - exfalso. destruct H0; auto.
+    - destruct H as (?&?&?).
+      rewrite Hfind in H. inv H.
+      exists (PS.remove y x); split; auto.
+      apply PSF.remove_2; auto.
+  Qed.
+
+  Fact has_arc_has_trans_arc : forall a a' x y,
+      (forall x y, has_arc a x y <-> has_arc a' x y) ->
+      has_trans_arc a x y <-> has_trans_arc a' x y.
+  Proof.
+    intros * Ha; split; intros Hta; induction Hta.
+    1,3:left; rewrite Ha in *; auto.
+    1,2:eapply tn1_trans; eauto; rewrite Ha in *; auto.
+  Qed.
+
+  (* Lemma remove_arc_has_trans_arc1 : forall a x y x' y' , *)
+  (*     has_trans_arc (remove_arc x y a) x' y' -> *)
+  (*     has_trans_arc a x' y'. *)
+  (* Proof. *)
+  (*   intros * Ha. *)
+  (*   induction Ha. *)
+  (*   - left. apply remove_arc_spec in H as (?&?); auto. *)
+  (*   - eapply tn1_trans; eauto. *)
+  (*     apply remove_arc_spec in H as (?&?); auto. *)
+  (* Qed. *)
+
+  (* Lemma remove_arc_AcyGraph : forall {v a} x y, *)
+  (*     AcyGraph v a -> *)
+  (*     exists a', (forall x' y', has_arc a' x' y' <-> has_arc (remove_arc x y a) x' y') /\ *)
+  (*       AcyGraph v a'. *)
+  (* Proof. *)
+  (*   fix remove_arc_AcyGraph 5. *)
+  (*   intros * g. *)
+  (*   destruct g. *)
+  (*   - exists (Env.empty _); split. *)
+  (*     + unfold remove_arc. rewrite Env.gempty. reflexivity. *)
+  (*     + constructor. *)
+  (*   - specialize (remove_arc_AcyGraph _ _ x y g) as (a'&?&?). *)
+  (*     exists a'; split; auto. *)
+  (*   - specialize (remove_arc_AcyGraph _ _ x y g) as (a'&?&?). *)
+  (*     destruct (Decidable.dec_and _ _ (decidable_eq_ident x x0) (decidable_eq_ident y y0)). *)
+  (*     + destruct H5; subst. *)
+  (*       exists a'. split; auto. *)
+  (*       intros x' y'. repeat rewrite remove_arc_spec, add_arc_spec. *)
+  (*       split; [intros Ha|intros (?&?)]. *)
+  (*       * apply H3, remove_arc_spec in Ha as (?&?); auto. *)
+  (*       * rewrite H3, remove_arc_spec. split; auto. *)
+  (*         destruct H5 as [?|(?&?)]; subst; auto. *)
+  (*         exfalso. destruct H6; auto. *)
+  (*     + exists (add_arc x0 y0 a'). *)
+  (*       split. 2:constructor; auto. *)
+  (*       * intros x' y'. *)
+  (*         rewrite add_arc_spec, H3. *)
+  (*         repeat rewrite remove_arc_spec. rewrite add_arc_spec. *)
+  (*         split; intros; repeat destruct_conj_disj; eauto 10. *)
+  (*         split; [auto|]. *)
+  (*         apply Decidable.not_and; auto. apply decidable_eq_ident. *)
+  (*       * rewrite has_arc_has_trans_arc; auto. *)
+  (*         intros Ha. eapply H2, remove_arc_has_trans_arc1; eauto. *)
+  (* Qed. *)
+
+  Lemma subset_AcyGraph : forall v a (g : AcyGraph v a) a',
+      (forall x y, has_arc a' x y -> has_arc a x y) ->
+      exists a'', (forall x y, has_arc a'' x y <-> has_arc a' x y) /\
+        AcyGraph v a''.
+  Proof.
+    fix subset_AcyGraph 3.
+    intros * g * Hsub.
+    destruct g.
+    - exists (Env.empty _); split; auto.
+      intros *. split; intros; exfalso.
+      + destruct H as (?&Hmap&?). rewrite Env.Props.P.F.empty_mapsto_iff in Hmap; auto.
+      + apply Hsub in H. destruct H as (?&Hmap&?). rewrite Env.Props.P.F.empty_mapsto_iff in Hmap; auto.
+    - specialize (subset_AcyGraph _ _ g _ Hsub) as (a''&?&?).
+      exists a''; split; auto.
+    - assert (forall x0 y0 : ident, has_arc (remove_arc x y a') x0 y0 -> has_arc a x0 y0) as Hsub'.
+      { intros * Ha.
+        apply remove_arc_spec in Ha as (Ha&Hneq). apply Hsub in Ha.
+        apply add_arc_spec in Ha as [Ha|(?&?)]; subst; auto.
+        exfalso. destruct Hneq; auto.
+      }
+      specialize (subset_AcyGraph _ _ g _ Hsub') as (a''&Heq''&Hg'').
+      destruct (has_arc_dec a' x y).
+      + exists (add_arc x y a''). split; [|constructor]; auto.
+        * intros *.
+          rewrite add_arc_spec, Heq'', remove_arc_spec.
+          split; [intros [(?&?)|(?&?)]|intros ?]; subst; auto.
+          destruct (ident_eq_dec x x0), (ident_eq_dec y y0); subst; auto.
+        * intro contra.
+          apply H2.
+          erewrite has_arc_has_trans_arc in contra; [|eauto].
+          clear - contra Hsub'.
+          induction contra; auto.
+          eapply tn1_trans; eauto.
+      + exists a''. split; auto.
+        intros *.
+        rewrite Heq'', remove_arc_spec.
+        split; [intros (?&?)| intros ?]; auto.
+        split; auto.
+        destruct (ident_eq_dec x x0), (ident_eq_dec y y0); subst; auto.
+  Qed.
+
+End remove_arc.
